Sharding a distributed database (#35)
* [SI] initial draft of the specification.

* [SI] todo code file

* [SI] minor fix

* [SI] fix run spec and add code snippet proof

* [SI] todo example 1

* [SI] new specs

* [SI] new specs (fix typo)

* [SI] An implementation of snapshot isolation.

* [SI] add simple specs. minor fixes in specs. added api as class.

* [SI] added example of anomalie 1. fixed error in the SI implementation. added runner for example.

* [SI] fix the SI implementation for reads and improve SI implementation

* [SI] read-only anomalie example

* [SI] more examples implemented and some util factoring

* [SI] specs using local (cache) points-to connective.

* [SI] local specs simplified.

* Added some KVS_Init_Srv proposition, in order to initialise the server.

* Implementation folder containing some useful instances created

* Example 2 almost finished; added injectivity of the KVS_serialization as a prerequisite.

* Some bugs in the commit specification fixed, specs for util functions defined.

* Example2 finished, except for the part waiting on the wait_on_readT specification

* clean up for new specs

* New specs

* small fix

* minor fix

* can_commit is decideable

* CommitT and CommitU almost identical to previous versions

* wait spec

* Prove of the classical example

* wait_on_keyT specifications

* Admitted crashing parts of deprecated proof of example 7. To be treated later

* cleanup in example files

* moved proof sketches example7 and example8

* disjoint_writes example

* sequential_writes example, wait_spec not strong enough to finish it

* wait spec improved

* only_reads example

* wait spec + disjoint writes changes in the code

* clean up, not compiling atm.

* classical example up to date with generated code, compiling again

* function call example finished, waiting for read spec change

* [SI] improve implementation of read request handler.

* [SI] started sketching the resources and model.

* stronger wait_spec

* stronger wait_spec, proof admitted for now

* stronger wait_spec

* wait spec improved a little, read spec changed to return a serializable value

* sequential_writes example

* cleanup

* class for client specs and invariant

* more cleanup

* tried to use the new wait spec

* read spec returned to the old one

* wait spec proven

* disjoint writes without invariant

* function call example; minor changes to resources

* no serializability example

* causality example

* sharding api

* small bug fixes + some documentation

---------

Co-authored-by: Leon Gondelman <gondelman@cs.au.dk>
Co-authored-by: Léon <leon.ducruet@ens-lyon.fr>
Co-authored-by: Alnor <anders.alnor.mathiasen@gmail.com>

ml_sources/examples/reliable_communication/client_server_printing.ml
@@ -2,39 +2,48 @@ open Ast
 open !Serialization_code
 open !Network_util_code
 
+let b = ref false
 
 let __print_recv_msg deser sa msg () =
-  let (SADDR (s, i)) = sa in
-  match deser (fst msg) with
-  | InjL repl ->
-    Printf.printf "(%s, %d) ---received---> HNDSHK packet %s,%d: \n%!"
-      s i (fst repl) (snd repl)
-  | InjR (InjL _) ->
-    Printf.printf
-      "(%s, %d) ---received---> ACKID packet: %s.\n%!" s i (fst msg)
-  | InjR (InjR _) ->
-    Printf.printf
-      "(%s, %d) ---received---> SEQID packet: %s.\n%!" s i (fst msg)
+  if !b
+  then
+    let (SADDR (s, i)) = sa in
+    match deser (fst msg) with
+    | InjL repl ->
+      Printf.printf "(%s, %d) ---received---> HNDSHK packet %s,%d: \n%!"
+        s i (fst repl) (snd repl)
+    | InjR (InjL _) ->
+      Printf.printf
+        "(%s, %d) ---received---> ACKID packet: %s.\n%!" s i (fst msg)
+    | InjR (InjR _) ->
+      Printf.printf
+        "(%s, %d) ---received---> SEQID packet: %s.\n%!" s i (fst msg)
 
 let __print_send_msg ser sa bdy () =
-  let msg = ser bdy in
-  let (SADDR (s, i)) = sa in
-  match bdy with
-  | InjL init ->
-     Printf.printf "(%s, %d) <-----send----- HNDSHK packet %s,%d: \n%!"
-       s i (fst init) (snd init)
-  | InjR (InjL _) ->
-    Printf.printf
-      "(%s, %d) <-----send----- ACKID packet: %s.\n%!" s i msg
-  | InjR (InjR _) ->
-    Printf.printf
-      "(%s, %d) <-----send----- SEQID packet: %s.\n%!" s i msg
+  if !b
+  then
+    let msg = ser bdy in
+    let (SADDR (s, i)) = sa in
+    match bdy with
+    | InjL init ->
+      Printf.printf "(%s, %d) <-----send----- HNDSHK packet %s,%d: \n%!"
+        s i (fst init) (snd init)
+    | InjR (InjL _) ->
+      Printf.printf
+        "(%s, %d) <-----send----- ACKID packet: %s.\n%!" s i msg
+    | InjR (InjR _) ->
+      Printf.printf
+        "(%s, %d) <-----send----- SEQID packet: %s.\n%!" s i msg
 
 let __print_send_handshake_msg sa msg () =
-  let (SADDR (s, i)) = sa in
-     Printf.printf "(%s, %d) <-----send----- HNDSHK packet %s: \n%!"
-       s i msg
+  if !b
+  then
+    let (SADDR (s, i)) = sa in
+    Printf.printf "(%s, %d) <-----send----- HNDSHK packet %s: \n%!"
+      s i msg
 
 let __print_new_chan clt_addr () =
-  let (SADDR (s, i)) = clt_addr in
-  Printf.printf "New channel created associated with saddr (%s, %d)\n%!" s i
+  if !b
+  then
+    let (SADDR (s, i)) = clt_addr in
+    Printf.printf "New channel created associated with saddr (%s, %d)\n%!" s i
