ml_sources/examples/snapshot_isolation/examples/function_call/function_call_code.ml
@@ -1,0 +1,26 @@
+open !Ast
+open Serialization_code
+open Snapshot_isolation_code
+open Util_code
+
+let transaction1 cst =
+  start cst;
+  write cst "x" 42;
+  commitU cst
+
+let transaction2 cst f =
+  start cst;
+  let r = f "x" in
+  write cst "y" r;
+  commitU cst
+
+let transaction1_client caddr kvs_addr =
+  let cst = init_client_proxy int_serializer caddr kvs_addr in
+  transaction1 cst
+
+let transaction2_client caddr kvs_addr f =
+  let cst = init_client_proxy int_serializer caddr kvs_addr in
+  transaction2 cst f
+
+let server srv =
+  init_server int_serializer srv
