ml_sources/examples/snapshot_isolation/snapshot_isolation_code.mli
@@ -1,0 +1,11 @@
+
+open Ast
+type 'a connection_state
+
+val init_server : 'a serializer -> saddr -> unit
+val start : 'a connection_state -> unit
+val read : 'a connection_state -> string -> 'a option
+val write : 'a connection_state -> string -> 'a -> unit
+val commit : 'a connection_state -> bool
+val run : 'a connection_state -> ('a connection_state -> unit) -> bool
+val init_client_proxy : 'a serializer -> saddr -> saddr -> 'a connection_state
