aneris/examples/reliable_communication/lib/sharding/spec/api_spec.v
@@ -9,156 +9,88 @@ From aneris.examples.reliable_communication.lib.mt_server.spec
      Require Import api_spec.
 From aneris.aneris_lang.lib.serialization Require Import serialization_proof.
 From aneris.aneris_lang.program_logic Require Import lightweight_atomic.
+Import inject.
 
 Section Spec.
 
-  Context `{!anerisG Mdl Σ, !DBG Σ, !DB_params}.
+  Context `{!anerisG Mdl Σ, !DB_params, !DBG Σ}.
 
   Definition write_spec (wr : val) sa : iProp Σ :=
-    ∀ E k v (P Q : iProp Σ),
-    □ (⌜↑DB_inv_name ⊆ E⌝ -∗
-       ⌜k ∈ DB_keys⌝ -∗
-       {{{ P ∗
-           □ (P ={⊤, E}=∗ ∃ old, k ↦ₖ old ∗
-               ▷ (k ↦ₖ Some (SV_val v) ={E, ⊤}=∗ Q))
-       }}}
-         wr #k v @[ip_of_address sa]
-       {{{ RET #(); Q }}}).
-
-  Definition atomic_write_spec (wr : val) sa : iProp Σ :=
-    ∀ (E : coPset) (k : Key) (v : SerializableVal),
+    ∀ (E : coPset) (k : Key) v,
     ⌜↑DB_inv_name ⊆ E⌝ -∗
     ⌜k ∈ DB_keys⌝ -∗
     <<< ∀∀ old, k ↦ₖ old >>>
-      wr #k v @[ip_of_address sa] E
-    <<<▷ RET #(); k ↦ₖ Some (SV_val v) >>>.
-
-  Lemma get_atomic_write_spec wr sa :
-    write_spec wr sa -∗ atomic_write_spec wr sa.
-  Proof.
-    iIntros "#write" (E k v inv_name k_keys Φ) "!>HΦ".
-    wp_apply ("write" $! _ _ _ _ (Φ #()) with "[//] [//] [HΦ]");
-          last by iIntros "HΦ".
-    iSplitL "HΦ"; first iApply "HΦ".
-    by iIntros "!>HΦ".
-  Qed.
+      wr $k $v @[ip_of_address sa] E
+    <<<▷ RET #(); k ↦ₖ Some v >>>.
 
   Definition simplified_write_spec (wr : val) sa : iProp Σ := 
-    ∀ (v : SerializableVal) (old : option val) (k : Key), ⌜k ∈ DB_keys⌝ -∗
+    ∀ v old (k : Key), ⌜k ∈ DB_keys⌝ -∗
     {{{ k ↦ₖ old }}}
-      wr #k v @[ip_of_address sa]
-    {{{ RET #(); k ↦ₖ Some (SV_val v) }}}.
+      wr $k $v @[ip_of_address sa]
+    {{{ RET #(); k ↦ₖ Some v }}}.
 
   Lemma get_simplified_write_spec wr sa :
     write_spec wr sa -∗ simplified_write_spec wr sa.
   Proof.
     iIntros "#write" (v old k k_keys Φ) "!>k_old HΦ".
-    wp_apply ("write" $! ⊤ _ _ (k ↦ₖ old ∗ _)%I (Φ #())
-            with "[//] [//] [$k_old HΦ]"); last by iIntros "?".
-    iSplitL "HΦ"; first iApply "HΦ".
-    iIntros "!>(k_old & HΦ)!>".
+    wp_apply ("write" $! ⊤ with "[//] [//]").
+    iModIntro.
     iExists old.
     iFrame.
-    iNext.
-    iIntros "k_v!>".
-    by iApply "HΦ".
+    iIntros "!>k_v".
+    iApply ("HΦ" with "k_v").
   Qed.
 
   Definition read_spec (rd : val) sa : iProp Σ :=
-    ∀ E k (P : iProp Σ) (Q : option val → iProp Σ),
-    □ (⌜↑DB_inv_name ⊆ E⌝ -∗
-       ⌜k ∈ DB_keys⌝ -∗
-       {{{ P ∗
-           □ (P ={⊤, E}=∗ ∃ v, k ↦ₖ v ∗ ▷ (k ↦ₖ v ={E,⊤}=∗ Q v))
-       }}}
-         rd #k @[ip_of_address sa]
-       {{{ vo, RET vo; (∃ v, ⌜vo = SOMEV v⌝ ∗ Q (Some v)) ∨
-                       (⌜vo = NONEV⌝ ∗ Q None) }}}).
-
-  Definition atomic_read_spec (rd : val) sa : iProp Σ :=
     ∀ (E : coPset) (k : Key),
     ⌜↑DB_inv_name ⊆ E⌝ -∗
     ⌜k ∈ DB_keys⌝ -∗
     <<< ∀∀ v, k ↦ₖ v >>>
-      rd #k @[ip_of_address sa] E
-    <<<▷ ∃∃ vo, RET vo; k ↦ₖ v ∗ ((∃ a, ⌜vo = SOMEV a⌝ ∗ ⌜v = Some a⌝) ∨
-                                  (⌜vo = NONEV⌝ ∗ ⌜v = None⌝)) >>>.
-
-  Lemma get_atomic_read_spec rd sa :
-    read_spec rd sa -∗ atomic_read_spec rd sa.
-  Proof.
-    iIntros "#read" (E k inv_name k_keys Φ) "!>HΦ".
-    wp_apply ("read" $! _ _ _ (λ v, (∃ a, ⌜v = Some a⌝ ∗ Φ (SOMEV a)) ∨
-                       (⌜v = None⌝ ∗ Φ NONEV))%I with "[//] [//] [HΦ]").
-    {
-      iSplit; first iApply "HΦ".
-      iIntros "!>HΦ".
-      iMod "HΦ" as "(%v & k_v & HΦ)".
-      iModIntro.
-      iExists v.
-      iFrame.
-      iIntros "!>k_v".
-      case: v=>[a|];
-      [iMod ("HΦ" $! (InjRV a) with "[$k_v]") as "HΦ"; [|iModIntro];
-            iLeft; iExists a; by iSplit|
-       iMod ("HΦ" $! (InjLV #()) with "[$k_v]") as "HΦ"; [|iModIntro];
-            iRight; by iSplit].
-    }
-    iIntros "% [(%v & -> & [(% & %eq & HΦ)|(%abs & _)])|(-> & [(% & %abs & _)|
-              (% & HΦ)])]"; [by move: eq=>[<-]|done..].
-  Qed.
+      rd $k @[ip_of_address sa] E
+    <<<▷ RET $v; k ↦ₖ v >>>.
 
   Definition simplified_read_spec (rd : val) sa : iProp Σ := 
     ∀ (k : Key) v, ⌜k ∈ DB_keys⌝ -∗
     {{{ k ↦ₖ v }}}
-      rd #k @[ip_of_address sa]
-    {{{ vo, RET vo; k ↦ₖ v ∗ ((⌜vo = NONEV⌝ ∗ ⌜v = None⌝) ∨
-        (∃ a, ⌜vo = SOMEV a⌝ ∗ ⌜v = Some a⌝)) }}}.
+      rd $k @[ip_of_address sa]
+    {{{ RET $v; k ↦ₖ v }}}.
 
   Lemma get_simplified_read_spec rd sa :
     read_spec rd sa -∗ simplified_read_spec rd sa.
   Proof.
     iIntros "#read" (k v k_keys Φ) "!>k_v HΦ".
-    wp_apply ("read" $! ⊤ _ (k ↦ₖ v ∗ _)%I (λ v, (∃ a, ⌜v = Some a⌝ ∗ Φ (SOMEV a)) ∨
-                       (⌜v = None⌝ ∗ Φ NONEV))%I with "[//] [//] [$k_v HΦ]").
-    {
-      iSplit; first iApply "HΦ".
-      iIntros "!>(k_v & HΦ)".
-      iModIntro.
-      iExists v.
-      iFrame.
-      iIntros "!> k_v!>".
-      case: v=>[a|];[iLeft; iExists a|iRight];
-        (iSplit; [done|iApply "HΦ"]; iFrame); [iRight; iExists a|iLeft]; by iSplit.
-    }
-    iIntros "% [(% & -> & [(% & %eq & HΦ)|(%abs & _)])|(-> & [(% & %abs & _)|
-              (% & HΦ)])]"; [by move:eq=>[<-]|done..].
+    wp_apply ("read" $! ⊤ with "[//] [//]").
+    iModIntro.
+    iExists v.
+    iFrame.
+    iIntros "!>k_v".
+    iApply ("HΦ" with "k_v").
   Qed.
 
   Definition hash_spec (hashv : val) (hash : Key → nat) : iProp Σ :=
     ∀ (k : Key) sa, ⌜k ∈ DB_keys⌝ -∗
     {{{ True }}}
-      hashv #k @[ip_of_address sa]
+      hashv $k @[ip_of_address sa]
     {{{ RET #(hash k); True }}}.
 
   Definition init_server_spec
-    SrvInit srv_si (shards_si : list _) hash : iProp Σ :=
-    ∀ hashv addrs, ⌜is_list DB_addrs addrs⌝ -∗
+    SrvInit srv_si (shards_si : list _) : iProp Σ :=
+    ∀ hash addrs, ⌜is_list DB_addrs addrs⌝ -∗
     {{{
-      hash_spec hashv hash ∗
-      SrvInit ∗
+      hash_spec hash DB_hash ∗
       DB_addr ⤇ srv_si ∗
+      ([∗ list] i↦sa ∈ DB_addrs, ∃ sa_si, ⌜shards_si !! i = Some sa_si⌝ ∗
+          (snd sa) ⤇ sa_si) ∗
+      SrvInit ∗
       DB_addr ⤳ (∅, ∅) ∗
       free_ports (ip_of_address DB_addr) {[port_of_address DB_addr]} ∗
-      ([∗ list] i↦sa ∈ DB_addrs,
-          (∃ sa_si , ⌜(shards_si !! i) = (Some sa_si)⌝ ∗ (snd sa) ⤇ sa_si)) ∗
       ([∗ list] i↦sa ∈ DB_addrs, unallocated {[ (fst sa) ]}) ∗ 
       ([∗ list] i↦sa ∈ DB_addrs, (fst sa) ⤳ (∅, ∅)) ∗
       ([∗ list] i↦sa ∈ DB_addrs,
             free_ports (ip_of_address (fst sa)) {[port_of_address (fst sa)]})
     }}}
-      init_server (s_serializer DB_serialization) #DB_addr addrs hashv
-                                          @[ip_of_address DB_addr]
+      init_server (s_serializer DB_key_ser) (s_serializer DB_val_ser)
+          #DB_addr addrs hash @[ip_of_address DB_addr]
     {{{ RET #(); True }}}.
 
   Definition init_shard_spec ShardInit shard_si sa : iProp Σ :=
@@ -168,44 +100,44 @@ Section Spec.
       sa ⤳ (∅, ∅) ∗
       free_ports (ip_of_address sa) {[port_of_address sa]}
     }}}
-      init_shard (s_serializer DB_serialization) #sa @[ip_of_address sa]
+      init_shard (s_serializer DB_key_ser) (s_serializer DB_val_ser)
+          #sa @[ip_of_address sa]
     {{{ RET #(); True }}}.
 
-  Definition init_client_proxy_spec srv_si : iProp Σ :=
+  Definition init_client_spec srv_si : iProp Σ :=
     ∀ sa,
     {{{
+      DB_addr ⤇ srv_si ∗
       unallocated {[sa]} ∗
       sa ⤳ (∅, ∅) ∗
-      DB_addr ⤇ srv_si ∗
       free_ports (ip_of_address sa) {[port_of_address sa]}
     }}}
-      init_client_proxy (s_serializer DB_serialization) #sa #DB_addr
-          @[ip_of_address sa]
+      init_client (s_serializer DB_key_ser) (s_serializer DB_val_ser)
+          #sa #DB_addr @[ip_of_address sa]
     {{{ wr rd, RET (wr, rd); read_spec rd sa ∗ write_spec wr sa }}}.
 
 End Spec.
 
 Section Init.
 
-  Context `{!anerisG Mdl Σ, !DBPreG Σ, !DB_params}.
+  Context `{!anerisG Mdl Σ, !DB_params, !DBPreG Σ}.
 
-  Class DB_Init (hash : Key → nat) :=
+  Class DB_Init :=
     {
     DB_init_setup E :
-      (∀ k, k ∈ DB_keys → hash k < length DB_addrs)%nat →
       ↑DB_inv_name ⊆ E →
       ⊢ |={E}=>
-        ∃ (dbg : @DBG Σ) InitSrv
+        ∃ (dbg : DBG Σ) InitSrv
           (InitShards : list _) srv_si shards_si,
         ([∗ set] k ∈ DB_keys, k ↦ₖ None) ∗
         InitSrv ∗
-        @init_server_spec _ _ _ _ InitSrv srv_si shards_si hash ∗
-        @init_client_proxy_spec _ _ _ dbg _ srv_si ∗
-        ([∗ list] i↦sa ∈ DB_addrs, ∃ Init_sa,
-        ⌜(InitShards !! i) = Some Init_sa⌝ ∗ Init_sa) ∗
+        init_server_spec InitSrv srv_si shards_si ∗
+        init_client_spec srv_si ∗
+        ([∗ list] i↦sa ∈ DB_addrs, ∃ Init_sa, ⌜InitShards !! i = Some Init_sa⌝ ∗
+            Init_sa) ∗
         ([∗ list] i↦sa ∈ DB_addrs, ∃ Init_sa sa_si,
-        ⌜(InitShards !! i) = Some Init_sa⌝ ∗ ⌜(shards_si !! i) = Some sa_si⌝ ∗
-        @init_shard_spec _ _ _ _ Init_sa sa_si (snd sa));
+          ⌜(InitShards !! i) = Some Init_sa⌝ ∗ ⌜(shards_si !! i) = Some sa_si⌝ ∗
+          init_shard_spec Init_sa sa_si (snd sa));
     }.
 
 End Init.
