aneris/examples/reliable_communication/lib/sharding/proof/proof_of_db_init.v
@@ -3,7 +3,7 @@ From aneris.examples.reliable_communication.lib.sharding.spec
     Require Import resources api_spec.
 From aneris.examples.reliable_communication.lib.sharding.proof
     Require Import proof_of_server_handler proof_of_client_handler
-              proof_of_init_server proof_of_init_shard proof_of_init_client_proxy.
+              proof_of_init_server proof_of_init_shard proof_of_init_client.
 From aneris.aneris_lang Require Import resources proofmode.
 From aneris.examples.reliable_communication.lib.mt_server Require Import
                     mt_server_code user_params.
@@ -20,25 +20,25 @@ Import lock_proof.
 
 Section utils.
 
-  Lemma init_shards `{!anerisG Mdl Σ, !DBG Σ, !DB_params, !SpecChanG Σ} γs E :
+  Lemma init_shards `{!anerisG Mdl Σ, !DB_params, !DBG Σ, !SpecChanG Σ} γs E :
       ↑DB_inv_name ⊆ E → length γs = length DB_addrs →
     ⊢ |={E}=> ∃ (ShardsInit : list (iProp Σ)) (shards_si : list _) (MTRs : list _),
-      ([∗ list] k ↦ sa ∈ DB_addrs, ∃ ShardInit shard_si γ,
-          let MTS := (@user_params_at_shard _ _ _ _ _ γ sa.2) in
-          (@run_server_spec _ _ _ _ MTS ShardInit shard_si) ∗
-          ⌜ShardsInit !! k = Some ShardInit⌝ ∗ ⌜shards_si !! k = Some shard_si⌝ ∗
-        ⌜γs !! k = Some γ⌝) ∗
-      ([∗ list] k ↦ sa ∈ DB_addrs, ∃ MTR γ,
-          let MTS := (@user_params_at_shard _ _ _ _ _ γ sa.2) in
-          (@make_request_spec _ _ _ _ MTS MTR)
-        ∗ ⌜γs !! k = Some γ⌝ ∗ ⌜MTRs !! k = Some MTR⌝) ∗
-      ([∗ list] k ↦ sa ∈ DB_addrs, ∃ MTR shard_si γ,
-          let MTS := (@user_params_at_shard _ _ _ _ _ γ sa.2) in
-          (@init_client_proxy_spec _ _ _ _ MTS
-       MTR shard_si) ∗ ⌜γs !! k = Some γ⌝ ∗ ⌜MTRs !! k = Some MTR⌝ ∗
-            ⌜shards_si !! k = Some shard_si⌝) ∗
-      ([∗ list] k ↦ sa ∈ DB_addrs, ∃ ShardInit, ShardInit ∗
-                    ⌜ShardsInit !! k = Some ShardInit⌝).
+      ([∗ list] i ↦ sa ∈ DB_addrs, ∃ ShardInit shard_si γ,
+          let MTS := user_params_at_shard γ sa.2 in
+          run_server_spec ShardInit shard_si ∗
+          ⌜ShardsInit !! i = Some ShardInit⌝ ∗ ⌜shards_si !! i = Some shard_si⌝ ∗
+        ⌜γs !! i = Some γ⌝) ∗
+      ([∗ list] i ↦ sa ∈ DB_addrs, ∃ MTR γ,
+          let MTS := user_params_at_shard γ sa.2 in
+          (@make_request_spec _ _ _ _ _ MTR)
+        ∗ ⌜γs !! i = Some γ⌝ ∗ ⌜MTRs !! i = Some MTR⌝) ∗
+      ([∗ list] i ↦ sa ∈ DB_addrs, ∃ MTR shard_si γ,
+          let MTS := user_params_at_shard γ sa.2 in
+          (@init_client_proxy_spec _ _ _ _ _ MTR shard_si) ∗
+            ⌜γs !! i = Some γ⌝ ∗ ⌜MTRs !! i = Some MTR⌝ ∗
+            ⌜shards_si !! i = Some shard_si⌝) ∗
+      ([∗ list] i ↦ sa ∈ DB_addrs, ∃ ShardInit,
+        ⌜ShardsInit !! i = Some ShardInit⌝ ∗ ShardInit).
   Proof.
     iIntros (H0).
     iRevert (γs).
@@ -48,7 +48,7 @@ Section utils.
     iMod ("Hind" $! γs len_γs) as "(%ShardsInit & %shards_si & %MTRs &
                   #run_shards & #request_shards & #init_shards_clt & ShardsInit)".
     iClear "Hind".
-    set (MTS := @user_params_at_shard _ _ _ _ _ γ addr.2).
+    set (MTS := user_params_at_shard γ addr.2).
     iMod (MTS_init_setup E MTS)
           as "(%shard_si & %ShardInit & %MTR & ShardInit &
                 #run_shard & #init_shard_clt & #request_shard)";
@@ -70,12 +70,12 @@ End utils.
 
 Section Init.
 
-  Context `{!anerisG Mdl Σ, !DBPreG Σ, !DB_params, !SpecChanG Σ}.
+  Context `{!anerisG Mdl Σ, !DB_params, !DBPreG Σ, !SpecChanG Σ}.
 
-  Global Instance db_init hash : DB_Init hash.
+  Global Instance db_init : DB_Init.
   Proof.
-    constructor=>E hash_valid name.
-    iMod (alloc_db _ hash_valid) as "(%dbg & %γs & %len_γs & %shards_valid
+    constructor=>E name.
+    iMod alloc_db as "(%dbg & %γs & %len_γs & %shards_valid
                               & ●_γs & ◯_γs)".
     iMod (MTS_init_setup E (@user_params_at_server _ _ _ _ dbg))
         as "(%srv_si & %SrvInit & %srv_MTR & SrvInit &
@@ -89,29 +89,16 @@ Section Init.
           (gset_to_gmap None DB_keys))%I) ShardsInit),
           srv_si, shards_si.
     iFrame.
-    iSplitR.
-    {
-      iIntros (shardsv addrs addrs_def Φ) "!>(#shards_spec & SrvInit & #srv_si &
-                        addr_∅ & addr_free & #shards_si & srv_unalloc & srv_∅ &
-                        srv_free) HΦ".
-      wp_apply (init_server_spec_holds with "[//] [//] []
-                 [$shards_spec $srv_si $addr_∅ $addr_free $shards_si
-                  $srv_unalloc $srv_∅ $srv_free $run_srv $init_shards_clt
-                  $request_shards $SrvInit]"); last done.
-      by iPureIntro=>k γ/shards_valid.
-    }
-    iSplitR.
-    {
-      iIntros (sa Φ) "!>(unalloc & ∅ & #srv_si & free) HΦ".
-      by wp_apply (init_client_proxy_spec_holds with "[$unalloc $∅ $srv_si $free
-                          $request_srv $init_srv_clt]").
-    }
+    iSplitR; first iApply (init_server_spec_holds with
+                            "[//] run_srv init_shards_clt request_shards").
+    iSplitR; first iApply (init_client_spec_holds with
+                            "request_srv init_srv_clt").
     iSplitL "●_γs ShardsInit".
     {
       iPoseProof (big_sepL_sep_2 with "●_γs ShardsInit") as "ShardsInit".
       iApply (big_sepL_impl with "ShardsInit").
-      iIntros "!>%i %sa %addrs_x ((%γ & %γs_γ & ●_γ) &
-              (%ShardInit & ShardInit & %ShardsInit_ShardInit))".
+      iIntros "!>%i %sa %addrs_sa ((%γ & %γs_γ & ●_γ) &
+              (%ShardInit & %ShardsInit_ShardInit & ShardInit))".
       iExists (∃ γ : gname, ⌜γs !! i = Some γ⌝ ∗ ShardInit ∗
            shard_mem γ (gset_to_gmap None DB_keys))%I.
       iFrame.
@@ -145,11 +132,11 @@ Section Init.
       by rewrite ShardsInit_ShardInit=>[][<-][->->].
     }
     iSplit; first done.
-    iIntros (Φ) "!>((%γ' & %γs_γ' & ShardInit & ●_γ') & #shard_si & ∅ & free) HΦ".
+    iIntros "!>%Φ ((%γ' & %γs_γ' & ShardInit & ●_γ') & #shard_si & ∅ & free) HΦ".
     rewrite γs_γ in γs_γ'.
     move:γs_γ'=>[<-].
-    by wp_apply (init_shard_spec_holds with "[$●_γ' $shard_si $∅ $free
-                            $run_shard $ShardInit]").
+    by wp_apply (init_shard_spec_holds with
+      "run_shard shard_si [$●_γ' $∅ $free $ShardInit]").
   Qed.
 
 End Init.
