aneris/examples/reliable_communication/lib/sharding/proof/proof_of_init_client.v
@@ -1,0 +1,90 @@
+From aneris.examples.reliable_communication.lib.sharding Require Import sharding_code.
+From aneris.examples.reliable_communication.lib.sharding.spec
+    Require Import resources api_spec.
+From aneris.aneris_lang Require Import resources proofmode.
+From aneris.examples.reliable_communication.lib.mt_server Require Import
+                    mt_server_code user_params.
+From aneris.aneris_lang.lib Require Import lock_proof.
+From aneris.examples.reliable_communication.lib.mt_server.spec
+     Require Import api_spec.
+From aneris.examples.reliable_communication.lib.mt_server.proof Require Import
+                    mt_server_proof.
+From aneris.aneris_lang.lib.serialization Require Import serialization_proof.
+Import sharding_code.
+Import inject.
+
+Section proof.
+
+  Context `{!anerisG Mdl Σ, !DB_params, !DBG Σ, !MTS_resources}.
+
+  Lemma init_client_spec_holds srv_si :
+    make_request_spec -∗
+    init_client_proxy_spec srv_si -∗
+    init_client_spec srv_si.
+  Proof.
+    iIntros "#request_srv #init_clt".
+    iIntros (sa) "!>%Φ (#srv_si & unalloc & ∅ & free) HΦ".
+    rewrite/init_client.
+    wp_pures.
+    wp_apply ("init_clt" with "[$unalloc $∅ $srv_si $free]").
+    iIntros (rpc) "CanRequest".
+    wp_pures.
+    wp_apply (newlock_spec DB_inv_name with "CanRequest").
+    iIntros (lk lock) "#lock".
+    wp_pures.
+    iApply "HΦ".
+    iSplit.
+    {
+      iIntros (E k inv_name k_keys Ψ) "!>HΨ".
+      wp_pures.
+      wp_apply (acquire_spec with "lock").
+      iIntros "% (-> & locked & CanRequest)".
+      wp_pures.
+      wp_apply ("request_srv" $! _ _ _ (inr (E, (λ vo, Ψ $vo)%I, k))
+          with "[$CanRequest HΨ]").
+      {
+        iSplit.
+        { iPureIntro=>/=. exists $k. right. split=>//=.
+            apply DB_keys_serializable. }
+        iRight.
+        iExists E, _, k.
+        iFrame.
+        by do 3 (iSplit; first done).
+      }
+      iIntros (repd repv) "(CanRequest & [(% & % & % & % & _ & _ & %)|
+          (% & % & % & %eq & % & -> & HΨ)])"; first done.
+      move: eq=>[_ <- _].
+      wp_pures.
+      wp_apply (release_spec with "[$lock $locked $CanRequest]").
+      iIntros (? ->).
+      wp_pures.
+      iApply "HΨ".
+    }
+    iIntros (E k v inv_name k_keys Ψ) "!>HΨ".
+    wp_pures.
+    wp_apply (acquire_spec with "lock").
+    iIntros "% (-> & locked & CanRequest)".
+    wp_pures.
+    wp_apply ("request_srv" $! _ _ _ (inl (E, Ψ #(), k, v))
+            with "[$CanRequest HΨ]").
+    {
+      iSplitR.
+      { iPureIntro=>/=. exists ($k, $v)%V. left. split=>//=. exists $k, $v.
+        split=>//=. split;
+          [apply DB_keys_serializable|apply DB_vals_serializable]. }
+      iLeft.
+      iExists E, (Ψ #()), k, v.
+      iFrame.
+      by do 3 (iSplit; first done).
+    }
+    iIntros (repd repv) "(CanRequest & [(% & % & % & % & HΨ & -> & %eq)|
+        (% & % & % & % & _)])"; last done.
+    move: eq => [_ <- _ _].
+    wp_pures.
+    wp_apply (release_spec with "[$lock $locked $CanRequest]").
+    iIntros (? ->).
+    wp_pures.
+    iApply "HΨ".
+  Qed.
+
+End proof.
