aneris/examples/snapshot_isolation/examples/function_call/function_call_proof.v
@@ -1,0 +1,361 @@
+From aneris.aneris_lang Require Import network resources proofmode.
+From aneris.aneris_lang.lib.serialization
+     Require Import serialization_proof.
+From aneris.examples.snapshot_isolation.specs
+     Require Import user_params resources specs.
+From aneris.aneris_lang.lib Require Import inject.
+From aneris.aneris_lang Require Import tactics proofmode adequacy.
+From trillium.prelude Require Import finitary.
+From aneris.aneris_lang.program_logic Require Import
+     aneris_weakestpre aneris_adequacy aneris_lifting.
+From iris.base_logic.lib Require Import invariants.
+From aneris.examples.snapshot_isolation.examples.function_call
+      Require Import function_call_code.
+Import ser_inj.
+From aneris.examples.snapshot_isolation.instantiation
+     Require Import snapshot_isolation_api_implementation.
+From aneris.examples.snapshot_isolation.util Require Import util_proof.
+From aneris.examples.snapshot_isolation Require Import snapshot_isolation_code.
+
+Definition server_addr := SocketAddressInet "0.0.0.0" 80.
+Definition client1_addr := SocketAddressInet "0.0.0.1" 80.
+Definition client2_addr := SocketAddressInet "0.0.0.2" 80.
+
+Instance params : User_params :=
+{| KVS_address := server_addr;
+  KVS_keys := {["x"; "y"]};
+  KVS_InvName := nroot .@ "siinv";
+  KVS_serialization := int_serialization;
+  KVS_ser_inj := int_ser_is_ser_injective;
+  KVS_ser_inj_alt := int_ser_is_ser_injective_alt
+|}.
+
+Definition client_inv_name := nroot.@"clinv".
+
+Section proof_of_code.
+
+  Context `{!anerisG Mdl Σ, !SI_resources Mdl Σ, !SI_client_toolbox}.
+
+  Definition f_spec (f : val) : iProp Σ :=
+    ∀ (k : Key) cst vo sa,
+    ⌜k ∈ KVS_keys⌝ -∗
+    {{{ k ↦{cst} vo }}}
+      f cst #k @[ip_of_address sa]
+    {{{ v', RET (SV_val v'); k ↦{cst} vo }}}.
+
+  Definition client_inv_def : iProp Σ :=
+    ∃ h, "x" ↦ₖ h.
+
+  Definition client_inv : iProp Σ :=
+    inv client_inv_name client_inv_def.
+
+  Lemma transaction1_spec :
+    ∀ (cst : val) sa,
+    client_inv -∗
+    {{{ ConnectionState cst CanStart }}}
+      transaction1 cst @[ip_of_address sa]
+    {{{ RET #(); True }}}.
+  Proof.
+    iIntros (cst sa) "#inv %Φ !> CanStart HΦ".
+    rewrite/transaction1.
+    wp_pures.
+    wp_apply (SI_start_spec $! _ _ (⊤ ∖ ↑client_inv_name)); first solve_ndisj.
+    iInv "inv" as ">(%h & x_h)" "close".
+    iModIntro.
+    iExists {[ "x" := h ]}.
+    iFrame.
+    iSplitL "x_h"; first iApply (big_sepM_singleton with "x_h").
+    iIntros "!>(Active & mem & cache & _)".
+    iPoseProof (big_sepM_insert with "mem") as "(x_h & _)"; first done.
+    iMod ("close" with "[x_h]") as "_".
+    { iNext. by iExists h. }
+    iPoseProof (big_sepM_insert with "cache") as "((x_h & x_upd) & _)"; first done.
+    iModIntro.
+    wp_pures.
+    wp_apply (SI_write_spec $! _ _ _ _ (SerVal #42) with "[] [$x_h $x_upd]");
+          first set_solver.
+    iIntros "(x_42 & x_upd)".
+    wp_pures.
+    wp_apply (commitU_spec _ _ (⊤ ∖ ↑client_inv_name)); first solve_ndisj.
+    iInv "inv" as ">(%h' & x_h')" "close".
+    iModIntro.
+    iExists {[ "x" := h' ]}, _, {[ "x" := (Some #42, true) ]}.
+    iFrame.
+    iSplitL "x_42 x_h' x_upd".
+    {
+      do 2 (iSplit; first by rewrite 2!dom_singleton_L).
+      iSplitL "x_h'"; first iApply (big_sepM_singleton with "x_h'").
+      iApply big_sepM_singleton.
+      iFrame.
+    }
+    iIntros "!>(CanStart & [(_ & mem)|(_ & mem)])".
+    {
+      iPoseProof (big_sepM2_insert with "mem") as "((x_42 & _) & _)";
+        [done..|].
+      iMod ("close" with "[x_42]") as "_".
+      { iNext. iExists _. iFrame. }
+      iModIntro.
+      iApply ("HΦ" with "[//]").
+    }
+    iPoseProof (big_sepM_insert with "mem") as "((x_h' & _) & _)"; first done.
+    iMod ("close" with "[x_h']") as "_".
+    { iNext. iExists h'. iFrame. }
+    iModIntro.
+    iApply ("HΦ" with "[//]").
+  Qed.
+
+  Lemma transaction2_spec :
+    ∀ (cst f : val) sa h,
+    f_spec f -∗
+    client_inv -∗
+    {{{ ConnectionState cst CanStart ∗ "y" ↦ₖ h }}}
+      transaction2 cst f @[ip_of_address sa]
+    {{{ RET #(); True }}}.
+  Proof.
+    iIntros (cst f sa hy) "#f_spec #inv %Φ !>(CanStart & y_hy) HΦ".
+    rewrite/transaction2.
+    wp_pures.
+    wp_apply (SI_start_spec $! _ _ (⊤ ∖ ↑client_inv_name)); first solve_ndisj.
+    iInv "inv" as ">(%hx & x_hx)" "close".
+    iModIntro.
+    iExists {[ "x" := hx; "y" := hy ]}.
+    iFrame.
+    iSplitL "x_hx y_hy".
+    {
+      iApply big_sepM_insert; first done.
+      iFrame.
+      iApply (big_sepM_singleton with "y_hy").
+    }
+    iIntros "!>(Active & mem & cache & _)".
+    iPoseProof (big_sepM_insert with "mem") as "(x_hx & mem)"; first done.
+    iPoseProof (big_sepM_insert with "mem") as "(y_hy & _)"; first done.
+    iMod ("close" with "[x_hx]") as "_".
+    { iNext. iExists hx. iFrame. }
+    iPoseProof (big_sepM_insert with "cache") as "((cache_x & x_upd) & cache)";
+        first done.
+    iPoseProof (big_sepM_insert with "cache") as "((cache_y & y_upd) & _)";
+        first done.
+    iModIntro.
+    wp_pures.
+    wp_apply ("f_spec" with "[] cache_x"); first set_solver.
+    iIntros (v') "cache_x".
+    wp_pures.
+    wp_apply (SI_write_spec with "[] [$cache_y $y_upd]"); first set_solver.
+    iIntros "(cache_y & y_upd)".
+    wp_pures.
+    wp_apply (commitU_spec _ _ (⊤ ∖ ↑client_inv_name)); first solve_ndisj.
+    iInv "inv" as ">(%hx' & x_hx')" "close".
+    iModIntro.
+    iExists {[ "x" := hx'; "y" := hy ]}, _,
+        {[ "x" := (hist_val hx, false); "y" := (Some (SV_val v'), true) ]}.
+    iFrame.
+    iSplitL "cache_x x_upd cache_y y_upd x_hx' y_hy".
+    {
+      rewrite !dom_insert_L !dom_empty_L.
+      do 2 (iSplit; first done).
+      by iSplitL "x_hx' y_hy";
+        repeat (iApply big_sepM_insert; first done; iFrame).
+    }
+    iIntros "!>(CanStart & [(_ & mem) | (_ & mem)])".
+    {
+      iPoseProof (big_sepM2_insert with "mem") as "((mem_x & _) & _)";
+          [done..|].
+      iMod ("close" with "[mem_x]") as "_".
+      { iNext. by iExists _. }
+      iApply ("HΦ" with "[//]").
+    }
+    iPoseProof (big_sepM_insert with "mem") as "((mem_x & _) & _)"; first done.
+    iMod ("close" with "[mem_x]") as "_".
+    { iNext. by iExists _. }
+    iApply ("HΦ" with "[//]").
+  Qed.
+
+  Lemma transaction1_client_spec :
+    ∀ clt,
+    client_inv -∗
+    {{{
+      clt ⤳ (∅, ∅) ∗
+      KVS_address ⤇ KVS_si ∗
+      unallocated {[clt]} ∗
+      free_ports (ip_of_address clt) {[port_of_address clt]}
+    }}}
+      transaction1_client #clt #KVS_address @[ip_of_address clt]
+    {{{ RET #(); True }}}.
+  Proof.
+    iIntros (clt) "#inv %Φ !> (∅ & #KVS_si & unalloc & free) HΦ".
+    rewrite/transaction1_client.
+    wp_pures.
+    wp_apply (SI_init_client_proxy_spec with "[$∅ $unalloc $free $KVS_si]").
+    iIntros (cst) "CanStart".
+    wp_pures.
+    by wp_apply (transaction1_spec with "inv CanStart").
+  Qed.
+
+  Lemma transaction2_client_spec :
+    ∀ clt f h,
+    client_inv -∗
+    f_spec f -∗
+    {{{
+      "y" ↦ₖ h ∗
+      clt ⤳ (∅, ∅) ∗
+      KVS_address ⤇ KVS_si ∗
+      unallocated {[clt]} ∗
+      free_ports (ip_of_address clt) {[port_of_address clt]}
+    }}}
+      transaction2_client #clt #KVS_address f @[ip_of_address clt]
+    {{{ RET #(); True }}}.
+  Proof.
+    iIntros (clt f h) "#inv #f_spec %Φ !> (y_h & ∅ & #KVS_si & unalloc & free) HΦ".
+    rewrite/transaction2_client.
+    wp_pures.
+    wp_apply (SI_init_client_proxy_spec with "[$∅ $unalloc $free $KVS_si]").
+    iIntros (cst) "CanStart".
+    wp_pures.
+    by wp_apply (transaction2_spec with "f_spec inv [$CanStart $y_h]").
+  Qed.
+
+  Lemma server_spec :
+    {{{
+      KVS_Init ∗
+      KVS_address ⤳ (∅, ∅) ∗
+      free_ports (ip_of_address KVS_address) {[port_of_address KVS_address]} ∗
+      KVS_address ⤇ KVS_si
+    }}}
+      server #KVS_address @[ip_of_address KVS_address]
+    {{{ RET #(); True }}}.
+  Proof.
+    iIntros (Φ) "(KVS_Init & ∅ & free & #KVS_si) HΦ".
+    rewrite/server.
+    wp_pures.
+    by wp_apply (SI_init_kvs_spec with "[$KVS_si $KVS_Init $∅ $free]").
+  Qed.
+
+End proof_of_code.
+
+Section proof_of_runner.
+
+  Context `{!anerisG Mdl Σ, !SI_init, !KVSG Σ}.
+
+  Definition f : val :=
+    λ: "cst" "k",
+      match: read "cst" "k" with
+          SOME "v" => "v"
+        | NONE     => #0
+      end.
+
+  Lemma f_spec_holds `{!SI_resources Mdl Σ, !SI_client_toolbox} :
+    ⊢ f_spec f.
+  Proof.
+    iIntros (k cst vo sa k_keys Φ) "!>k_vo HΦ".
+    rewrite/f.
+    wp_pures.
+    wp_apply (SI_read_spec with "[//] k_vo").
+    iIntros "k_vo".
+    case: vo=>[v|].
+    {
+      iMod (OwnLocalKey_serializable $! SI_GlobalInv with "k_vo")
+        as "(k_vo & %v_ser)"; first done.
+      wp_pures.
+      by iApply ("HΦ" $! (SerVal v)).
+    }
+    wp_pures.
+    by iApply ("HΦ" $! (SerVal #0)).
+  Qed.
+
+  Definition runner : expr :=
+    Start "0.0.0.0" (server #KVS_address) ;;
+    Start "0.0.0.1" (transaction1_client #client1_addr #KVS_address) ;;
+    Start "0.0.0.2" (transaction2_client #client2_addr #KVS_address f).
+
+  Lemma runner_spec :
+    {{{
+      server_addr ⤳ (∅, ∅) ∗
+      client1_addr ⤳ (∅, ∅) ∗
+      client2_addr ⤳ (∅, ∅) ∗
+      unallocated {[server_addr]} ∗
+      unallocated {[client1_addr]} ∗
+      unallocated {[client2_addr]} ∗
+      free_ip (ip_of_address server_addr) ∗
+      free_ip (ip_of_address client1_addr) ∗
+      free_ip (ip_of_address client2_addr)
+    }}}
+      runner @["system"]
+    {{{ RET #(); True }}}.
+  Proof.
+    iIntros (Φ) "(srv_∅ & clt1_∅ & clt2_∅ & srv_unalloc & clt1_unalloc &
+            clt2_unalloc & srv_free & clt1_free & clt2_free) HΦ".
+    rewrite/runner.
+    iMod SI_init_module as "(% & % & mem & KVS_Init)".
+    iPoseProof (big_sepS_insert with "mem") as "(x_mem & mem)"; first done.
+    iPoseProof (big_sepS_delete _ _ "y" with "mem") as "(y_mem & _)";
+      first set_solver.
+    iMod (inv_alloc client_inv_name _ client_inv_def with "[x_mem]") as "#inv".
+    { iNext. by iExists _. }
+    wp_apply (aneris_wp_socket_interp_alloc_singleton KVS_si with "srv_unalloc").
+    iIntros "#KVS_si".
+    wp_apply (aneris_wp_start {[80%positive]}).
+    iSplitL "srv_free"; first done.
+    iSplitR "KVS_Init srv_∅"; last first.
+    { iIntros "!>free". by wp_apply (server_spec with "[$]"). }
+    iNext.
+    wp_pures.
+    wp_apply (aneris_wp_start {[80%positive]}).
+    iSplitL "clt1_free"; first done.
+    iSplitR "clt1_∅ clt1_unalloc"; last first.
+    {
+      iIntros "!>free".
+      by wp_apply (transaction1_client_spec client1_addr with "inv [$]").
+    }
+    iNext.
+    wp_pures.
+    wp_apply (aneris_wp_start {[80%positive]}).
+    iSplitL "clt2_free"; first done.
+    iSplitR "clt2_∅ clt2_unalloc y_mem"; last first.
+    {
+      iIntros "!>free".
+      by wp_apply (transaction2_client_spec client2_addr with "inv [] [$]");
+        first iApply f_spec_holds.
+    }
+    iNext.
+    by iApply "HΦ".
+  Qed.
+
+End proof_of_runner.
+
+Definition unit_model := model _ (λ _ _, False) ().
+
+Lemma unit_model_rel_finitary : aneris_model_rel_finitary unit_model.
+Proof. intros ?. apply finite_smaller_card_nat. apply _. Qed.
+
+Definition ips : gset ip_address :=
+  {[ ip_of_address server_addr ; ip_of_address client1_addr
+  ; ip_of_address client2_addr ]}.
+
+Definition sa_dom : gset socket_address :=
+  {[ server_addr ; client1_addr; client2_addr ]}.
+
+Definition init_state :=
+  {|
+    state_heaps := {["system" := ∅ ]};
+    state_sockets := {["system" := ∅ ]};
+    state_ms := ∅;
+  |}.
+
+Theorem runner_safe :
+  aneris_adequate runner "system" init_state (λ _, True).
+Proof.
+  set (Σ := #[anerisΣ unit_model; KVSΣ]).
+  apply (@adequacy Σ unit_model _ _ ips sa_dom ∅ ∅ ∅);
+    [apply unit_model_rel_finitary|move=>?|set_solver..].
+  iIntros "!> Hunallocated Hhist Hfrag Hips Hlbl _ _ _ _".
+  iApply (runner_spec with "[Hunallocated Hhist Hfrag Hips Hlbl]" ).
+  2 : { iModIntro. done. }
+  do 2 (iDestruct (unallocated_split with "Hunallocated") as "[Hunallocated ?]";
+  [set_solver|]). iFrame.
+  do 2 (rewrite big_sepS_union; [|set_solver];
+  rewrite !big_sepS_singleton;
+  iDestruct "Hhist" as "[Hhist ?]"; iFrame).
+  do 2 (rewrite big_sepS_union; [|set_solver];
+  rewrite !big_sepS_singleton;
+  iDestruct "Hips" as "[Hips ?]"; iFrame).
+Qed.
