aneris/examples/snapshot_isolation/examples/no_serializability/no_serializability_proof.v
@@ -1,0 +1,1048 @@
+From aneris.aneris_lang Require Import network resources proofmode.
+From aneris.aneris_lang.lib Require Import
+     list_proof inject lock_proof.
+From aneris.aneris_lang.lib.serialization
+     Require Import serialization_proof.
+From aneris.aneris_lang.program_logic Require Import lightweight_atomic.
+From aneris.examples.snapshot_isolation.specs
+     Require Import user_params resources specs.
+From aneris.aneris_lang Require Import tactics proofmode adequacy.
+From trillium.prelude Require Import finitary.
+From aneris.aneris_lang.program_logic Require Import
+     aneris_weakestpre aneris_adequacy aneris_lifting.
+From iris.base_logic.lib Require Import invariants.
+From aneris.examples.snapshot_isolation.examples.no_serializability
+      Require Import no_serializability_code.
+Import ser_inj.
+Import network_util_proof.
+From aneris.examples.snapshot_isolation.instantiation
+     Require Import snapshot_isolation_api_implementation.
+From aneris.examples.snapshot_isolation.util Require Import util_proof.
+
+Definition server_addr := SocketAddressInet "0.0.0.0" 80.
+Definition client_1_addr := SocketAddressInet "0.0.0.1" 80.
+Definition client_2_addr := SocketAddressInet "0.0.0.2" 80.
+Definition client_3_addr := SocketAddressInet "0.0.0.3" 80.
+Definition client_4_addr := SocketAddressInet "0.0.0.4" 80.
+
+Instance params : User_params :=
+{| KVS_address := server_addr;
+  KVS_keys := {["x"; "y"; "z"]};
+  KVS_InvName := nroot .@ "siinv";
+  KVS_serialization := int_serialization;
+  KVS_ser_inj := int_ser_is_ser_injective;
+  KVS_ser_inj_alt := int_ser_is_ser_injective_alt
+|}.
+
+Definition client_inv_name := nroot.@"clinv".
+
+Section proofs.
+
+Context `{!anerisG Mdl Σ, !SI_resources Mdl Σ, !SI_client_toolbox}.
+
+  Definition client_inv_def : iProp Σ :=
+  ∃ hx hy hz, "x" ↦ₖ hx ∗ "y" ↦ₖ hy ∗ "z" ↦ₖ hz ∗
+    ((⌜hx = []⌝ ∗ ⌜hy = []⌝ ∗ ⌜hz = []⌝) ∨
+      (⌜#1 ∈ hz⌝ ∗ ∃ vx vy, ⌜hist_val hx = Some vx⌝ ∗ ⌜hist_val hy = Some vy⌝ ∗
+      (⌜vx = #1⌝ ∨ ⌜vx = #(-1)⌝) ∗(⌜vy = #1⌝ ∨ ⌜vy = #(-1)⌝))).
+
+  Definition client_inv : iProp Σ :=
+    inv client_inv_name client_inv_def.
+
+  Lemma transaction1_spec :
+    ∀ cst sa,
+    client_inv -∗
+    {{{ ConnectionState cst CanStart }}}
+      transaction1 cst @[ip_of_address sa]
+    {{{ RET #(); True }}}.
+  Proof.
+    iIntros (cst sa) "#inv %Φ !>CanStart HΦ".
+    rewrite/transaction1.
+    wp_pures.
+    wp_apply (SI_start_spec $! _ _ (⊤ ∖ ↑client_inv_name));
+      first solve_ndisj.
+    iInv "inv" as ">(%hx & %hy & %hz & x_hx & y_hy & z_hz & init)" "close".
+    iModIntro.
+    iExists {[ "x" := hx; "y" := hy; "z" := hz ]}.
+    iFrame.
+    iSplitL "x_hx y_hy z_hz";
+      first by repeat (iApply big_sepM_insert; first done; iFrame).
+    iIntros "!>(Active & mem & cache & _)".
+    iMod ("close" with "[mem init]") as "_".
+    {
+      iNext.
+      iExists hx, hy, hz.
+      repeat (iPoseProof (big_sepM_insert with "mem") as "(k_hk & mem)";
+                first done; iFrame).
+    }
+    iModIntro.
+    wp_pures.
+    iPoseProof (big_sepM_insert with "cache") as "((x_hx & x_upd) & cache)";
+      first done.
+    iPoseProof (big_sepM_insert with "cache") as "((y_hy & y_upd) & cache)";
+      first done.
+    iPoseProof (big_sepM_insert with "cache") as "((z_hz & z_upd) & _)";
+      first done.
+    wp_apply (SI_write_spec $! _ _ _ _ (SerVal #1) with "[] [$x_hx $x_upd]");
+      first set_solver.
+    iIntros "(x_1 & x_upd)".
+    wp_pures.
+    wp_apply (SI_write_spec $! _ _ _ _ (SerVal #1) with "[] [$y_hy $y_upd]");
+      first set_solver.
+    iIntros "(y_1 & y_upd)".
+    wp_pures.
+    wp_apply (SI_write_spec $! _ _ _ _ (SerVal #1) with "[] [$z_hz $z_upd]");
+      first set_solver.
+    iIntros "(z_1 & z_upd)".
+    wp_pures.
+    wp_apply (commitU_spec _ _ (⊤ ∖ ↑client_inv_name)); first solve_ndisj.
+    iInv "inv" as ">(%hx' & %hy' & %hz' & x_hx' & y_hy' & z_hz' & #init)" "close".
+    iModIntro.
+    iExists {[ "x" := hx'; "y" := hy'; "z" := hz' ]}, _,
+      {[ "x" := (Some #1, true); "y" := (Some #1, true); "z" := (Some #1, true) ]}.
+    iFrame.
+    iSplitL "x_1 y_1 z_1 x_hx' y_hy' z_hz' x_upd y_upd z_upd".
+    {
+      rewrite !dom_insert_L !dom_empty_L.
+      do 2 (iSplit; first done).
+      by iSplitL "x_hx' y_hy' z_hz'";
+        repeat (iApply big_sepM_insert; first done; iFrame).
+    }
+    have x_key : "x" ∈ KVS_keys by set_solver.
+    have y_key : "y" ∈ KVS_keys by set_solver.
+    have z_key : "z" ∈ KVS_keys by set_solver.
+    iIntros "!>(CanStart & [(%can_commit & mem)|(_ & mem)])";
+      (iMod ("close" with "[mem]") as "_"; last by iApply "HΦ").
+    {
+      iPoseProof (big_sepM2_insert with "mem") as "((x_1 & _) & mem)"; [done..|].
+      iPoseProof (big_sepM2_insert with "mem") as "((y_1 & _) & mem)"; [done..|].
+      iPoseProof (big_sepM2_insert with "mem") as "((z_1 & _) & _)"; [done..|].
+      rewrite bool_decide_spec in can_commit.
+      move: (can_commit _ x_key).
+      rewrite lookup_insert bool_decide_spec !lookup_insert=>[][->].
+      move: (can_commit _ y_key).
+      rewrite lookup_insert_ne// lookup_insert bool_decide_spec lookup_insert_ne//
+          lookup_insert lookup_insert_ne// lookup_insert=>[][->].
+      move: (can_commit _ z_key).
+      rewrite lookup_insert_ne// lookup_insert_ne// lookup_insert bool_decide_spec
+            lookup_insert_ne// lookup_insert_ne// lookup_insert
+            lookup_insert_ne// lookup_insert_ne// lookup_insert=>[][->].
+      iNext.
+      iExists (#1 :: hx), (#1 :: hy), (#1 :: hz).
+      iFrame.
+      iPureIntro.
+      right.
+      split; first repeat constructor.
+      exists #1, #1.
+      do 2 (split; first done).
+      by split; left.
+    }
+    iPoseProof (big_sepM_insert with "mem") as "((x_hx' & _) & mem)"; first done.
+    iPoseProof (big_sepM_insert with "mem") as "((y_hy' & _) & mem)"; first done.
+    iPoseProof (big_sepM_insert with "mem") as "((z_hz' & _) & _)"; first done.
+    iNext.
+    iExists hx', hy', hz'.
+    iFrame "∗#".
+  Qed.
+
+  Lemma transaction2_spec :
+    ∀ cst sa,
+    client_inv -∗
+    {{{ ConnectionState cst CanStart }}}
+      transaction2 cst @[ip_of_address sa]
+    {{{ RET #(); True }}}.
+  Proof.
+    iIntros (cst sa) "#inv %Φ!>CanStart HΦ".
+    rewrite/transaction2.
+    wp_pures.
+    wp_apply (SI_start_spec $! _ _ (⊤ ∖ ↑client_inv_name)); first solve_ndisj.
+    iInv "inv" as ">(%hx & %hy & %hz & x_hx & y_hy & z_hz & init)" "close".
+    iModIntro.
+    iExists {[ "x" := hx; "y" := hy; "z" := hz ]}.
+    iFrame.
+    iSplitL "x_hx y_hy z_hz";
+      first by repeat (iApply big_sepM_insert; first done; iFrame).
+    iIntros "!>(Active & mem & cache & Seen)".
+    iMod ("close" with "[mem init]") as "_".
+    {
+      iNext.
+      iExists hx, hy, hz.
+      iPoseProof (big_sepM_insert with "mem") as "(x_hx & mem)"; first done.
+      iPoseProof (big_sepM_insert with "mem") as "(y_hy & mem)"; first done.
+      iPoseProof (big_sepM_insert with "mem") as "(z_hz & _)"; first done.
+      iFrame.
+    }
+    iModIntro.
+    wp_pures.
+    wp_apply (simplified_wait_on_keyT_spec _ _ #1 _ _ _ (⊤ ∖ ↑client_inv_name)
+        (λ m, ∃ hx hy hz vx vy, ⌜m !! "x" = Some hx⌝ ∗ ⌜m !! "y" = Some hy⌝ ∗
+          ⌜m !! "z" = Some hz⌝ ∗ ⌜#1 ∈ hz⌝ ∗
+          ⌜hist_val hx = Some vx⌝ ∗ ⌜hist_val hy = Some vy⌝ ∗
+          (⌜vx = #1⌝ ∨ ⌜vx = #(-1)⌝) ∗ (⌜vy = #1⌝ ∨ ⌜vy = #(-1)⌝))%I
+          emp emp with
+          "[] [] [] [] [] [] [$Active $cache $Seen]"); first solve_ndisj.
+    1, 2 : rewrite !dom_insert_L; iPureIntro; set_solver.
+    {
+      iIntros "!>%h (#Seen & _)".
+      iInv "inv" as ">(%hx' & %hy' & %hz' & x_hx' & y_hy' & z_hz' &
+          [(_ & _ & ->)|(%hz'_1 & (%vx & %vy & %hx'_vx & %hy'_vy & 
+            (%Hvx & %Hvy)))])" "close".
+      { iMod (Seen_valid with "[] [$Seen $z_hz']") as "(z_hz' & %abs)";
+          [solve_ndisj|iApply SI_GlobalInv|by apply suffix_nil_inv in abs].
+      }
+      iModIntro.
+      iExists {[ "x" := hx'; "y" := hy'; "z" := hz' ]}.
+      iSplit; first by rewrite !dom_insert_L.
+      iSplitL "x_hx' y_hy' z_hz'";
+        first by repeat (iApply big_sepM_insert; first done; iFrame).
+      iSplitR.
+      {
+        iExists hx', hy', hz', vx, vy.
+        iFrame "%".
+        by rewrite (lookup_insert_ne _ _ "y").
+      }
+      iSplitR; first done.
+      iIntros "!>(mem & _)".
+      iMod ("close" with "[mem]") as "_"; last done.
+      iNext.
+      iExists hx', hy', hz'.
+      iPoseProof (big_sepM_insert with "mem") as "(x_hx' & mem)"; first done.
+      iPoseProof (big_sepM_insert with "mem") as "(y_hy' & mem)"; first done.
+      iPoseProof (big_sepM_insert with "mem") as "(z_hz' & _)"; first done.
+      iFrame.
+      iRight.
+      iSplit; first done.
+      by iExists vx, vy.
+    }
+    {
+      iModIntro.
+      iInv "inv" as ">(%hx' & %hy' & %hz' & x_hx' & y_hy' & z_hz' &
+          %Hinv)" "close".
+      iModIntro.
+      iExists {[ "x" := hx'; "y" := hy'; "z" := hz' ]}.
+      iSplit; first by rewrite !dom_insert_L.
+      iSplitL "x_hx' y_hy' z_hz'";
+        first by repeat (iApply big_sepM_insert; first done; iFrame).
+      iIntros "!>mem".
+      iMod ("close" with "[mem]") as "_"; last done.
+      iNext.
+      iExists hx', hy', hz'.
+      iPoseProof (big_sepM_insert with "mem") as "(x_hx' & mem)"; first done.
+      iPoseProof (big_sepM_insert with "mem") as "(y_hy' & mem)"; first done.
+      iPoseProof (big_sepM_insert with "mem") as "(z_hz' & _)"; first done.
+      iFrame "∗ %".
+    }
+    {
+      iIntros (v' Ψ) "!>_ HΨ".
+      wp_pures.
+      wp_op; first apply bin_op_eval_eq_val.
+      iApply "HΨ".
+      by rewrite bool_decide_spec.
+    }
+    rewrite !dom_insert_L.
+    iClear (hx hy hz) "".
+    iIntros (m) "(%dom_m & (%hx & %hy & %hz & %vx & %vy & %m_x & %m_y & %m_z &
+          %hz_not_empty & %hx_vx & %hy_vy & %Hvx & %Hvy) & Active & cache & Seen)".
+    wp_pures.
+    iPoseProof (big_sepM_delete _ _ _ _ m_x with "cache") as
+        "((x_hx & x_upd) & cache)".
+    iPoseProof (big_sepM_delete _ _ "y" hy with "cache") as
+        "((y_hy & y_upd) & cache)"; first by rewrite lookup_delete_ne.
+    iPoseProof (big_sepM_delete _ _ "z" hz with "cache") as
+        "((z_hz & z_upd) & _)"; first by rewrite !lookup_delete_ne.
+    iPoseProof (big_sepM_lookup _ _ _ _ m_z with "Seen") as "#Seen_z".
+    wp_apply (SI_read_spec with "[] x_hx"); first set_solver.
+    iIntros "x_hx".
+    rewrite hx_vx hy_vy.
+    destruct Hvx as [-> | ->].
+    {
+      wp_pures.
+      wp_apply (SI_write_spec $! _ _ _ _ (SerVal #(-1)) with
+          "[] [$y_hy $y_upd]"); first set_solver.
+      iIntros "(y_1 & y_upd)".
+      wp_pures.
+      wp_apply (commitU_spec _ _ (⊤ ∖ ↑client_inv_name)); first solve_ndisj.
+      iInv "inv" as ">(%hx' & %hy' & %hz' & x_hx' & y_hy' & z_hz' &
+          [(_ & _ & ->)|(%hz'_not_empty & %vx' & %vy' & %hx'_vx' & 
+            %hy'_vy' & %Hvx' & %Hvy')])" "close".
+      {
+        iMod (Seen_valid $! SI_GlobalInv with "[$Seen_z $z_hz']") as
+            "(z_hz' & %abs)"; first solve_ndisj.
+        apply suffix_nil_inv in abs.
+        rewrite abs in hz_not_empty.
+        by apply elem_of_nil in hz_not_empty.
+      }
+      iModIntro.
+      iExists {[ "x" := hx'; "y" := hy'; "z" := hz' ]}, m,
+              {[ "x" := (Some #1, false); "y" := (Some #(-1), true);
+                  "z" := (hist_val hz, false) ]}.
+      iFrame.
+      iSplitL "x_hx x_hx' x_upd y_1 y_hy' y_upd z_hz z_hz' z_upd".
+      {
+        rewrite !dom_insert_L dom_m !dom_empty_L.
+        do 2 (iSplit; first done).
+        by iSplitL "x_hx' y_hy' z_hz'";
+            repeat (iApply big_sepM_insert; first done; iFrame).
+      }
+      iIntros "!>(_ & [(_ & mem)|(_ & mem)])".
+      {
+        iMod ("close" with "[mem]") as "_"; last by iApply "HΦ".
+        iPoseProof (big_sepM2_insert with "mem") as "((x_hx' & _) & mem)";
+          [done..|].
+        iPoseProof (big_sepM2_insert with "mem") as "((y_hy' & _) & mem)";
+          [done..|].
+        iPoseProof (big_sepM2_insert with "mem") as "((z_hz' & _) & _)";
+          [done..|].
+        have -> : commit_event (hist_val hz, false) hz' = hz'
+              by case: (hist_val hz).
+        iNext.
+        iExists hx', (#(-1) :: hy'), hz'.
+        iFrame.
+        iPureIntro.
+        right.
+        split; first done.
+        exists vx', #(-1).
+        do 2 (split; first done).
+        by split; last right.
+      }
+      iMod ("close" with "[mem]") as "_"; last by iApply "HΦ".
+      iPoseProof (big_sepM_insert with "mem") as "((x_hx' & _) & mem)";
+          first done.
+      iPoseProof (big_sepM_insert with "mem") as "((y_hy' & _) & mem)";
+          first done.
+      iPoseProof (big_sepM_insert with "mem") as "((z_hz' & _) & _)";
+          first done.
+      iNext.
+      iExists _, _, _.
+      iFrame.
+      iPureIntro.
+      right.
+      split; first done.
+      by exists vx', vy'.
+    }
+    wp_pures.
+    wp_apply (commitU_spec _ _ (⊤ ∖ ↑client_inv_name)); first solve_ndisj.
+    iInv "inv" as ">(%hx' & %hy' & %hz' & x_hx' & y_hy' & z_hz' &
+          %Hinv)" "close".
+    iModIntro.
+    iExists {[ "x" := hx'; "y" := hy'; "z" := hz' ]}, m,
+            {[ "x" := (Some #(-1), false); "y" := (Some vy, false);
+                "z" := (hist_val hz, false) ]}.
+    iFrame.
+    iSplitL "x_upd x_hx x_hx' y_upd y_hy y_hy' z_upd z_hz z_hz'".
+    {
+      rewrite !dom_insert_L dom_m !dom_empty_L.
+      do 2 (iSplit; first done).
+      by iSplitL "x_hx' y_hy' z_hz'";
+          repeat (iApply big_sepM_insert; first done; iFrame).
+    }
+    iIntros "!>(_ & [(_ & mem)|(_ & mem)])".
+    {
+      iMod ("close" with "[mem]") as "_"; last by iApply "HΦ".
+      iPoseProof (big_sepM2_insert with "mem") as "((x_hx' & _) & mem)";
+        [done..|].
+      iPoseProof (big_sepM2_insert with "mem") as "((y_hy' & _) & mem)";
+        [done..|].
+      iPoseProof (big_sepM2_insert with "mem") as "((z_hz' & _) & _)";
+        [done..|].
+      have -> : commit_event (hist_val hz, false) hz' = hz'
+            by case: (hist_val hz).
+      iNext.
+      iExists hx', hy', hz'.
+      by iFrame.
+    }
+    iMod ("close" with "[mem]") as "_"; last by iApply "HΦ".
+    iPoseProof (big_sepM_insert with "mem") as "((x_hx' & _) & mem)";
+      [done..|].
+    iPoseProof (big_sepM_insert with "mem") as "((y_hy' & _) & mem)";
+      [done..|].
+    iPoseProof (big_sepM_insert with "mem") as "((z_hz' & _) & _)";
+      [done..|].
+    iNext.
+    iExists _, _, _.
+    by iFrame.
+  Qed.
+
+  Lemma transaction3_spec :
+    ∀ cst sa,
+    client_inv -∗
+    {{{ ConnectionState cst CanStart }}}
+      transaction3 cst @[ip_of_address sa]
+    {{{ RET #(); True }}}.
+  Proof.
+    iIntros (cst sa) "#inv %Φ!>CanStart HΦ".
+    rewrite/transaction3.
+    wp_pures.
+    wp_apply (SI_start_spec $! _ _ (⊤ ∖ ↑client_inv_name)); first solve_ndisj.
+    iInv "inv" as ">(%hx & %hy & %hz & x_hx & y_hy & z_hz & init)" "close".
+    iModIntro.
+    iExists {[ "x" := hx; "y" := hy; "z" := hz ]}.
+    iFrame.
+    iSplitL "x_hx y_hy z_hz";
+      first by repeat (iApply big_sepM_insert; first done; iFrame).
+    iIntros "!>(Active & mem & cache & Seen)".
+    iMod ("close" with "[mem init]") as "_".
+    {
+      iNext.
+      iExists hx, hy, hz.
+      iPoseProof (big_sepM_insert with "mem") as "(x_hx & mem)"; first done.
+      iPoseProof (big_sepM_insert with "mem") as "(y_hy & mem)"; first done.
+      iPoseProof (big_sepM_insert with "mem") as "(z_hz & _)"; first done.
+      iFrame.
+    }
+    iModIntro.
+    wp_pures.
+    wp_apply (simplified_wait_on_keyT_spec _ _ #1 _ _ _ (⊤ ∖ ↑client_inv_name)
+        (λ m, ∃ hx hy hz vx vy, ⌜m !! "x" = Some hx⌝ ∗ ⌜m !! "y" = Some hy⌝ ∗
+          ⌜m !! "z" = Some hz⌝ ∗ ⌜#1 ∈ hz⌝ ∗
+          ⌜hist_val hx = Some vx⌝ ∗ ⌜hist_val hy = Some vy⌝ ∗
+          (⌜vx = #1⌝ ∨ ⌜vx = #(-1)⌝) ∗ (⌜vy = #1⌝ ∨ ⌜vy = #(-1)⌝))%I
+          emp emp with
+          "[] [] [] [] [] [] [$Active $cache $Seen]"); first solve_ndisj.
+    1, 2 : rewrite !dom_insert_L; iPureIntro; set_solver.
+    {
+      iIntros "!>%h (#Seen & _)".
+      iInv "inv" as ">(%hx' & %hy' & %hz' & x_hx' & y_hy' & z_hz' &
+          [(_ & _ & ->)|(%hz'_1 & (%vx & %vy & %hx'_vx & %hy'_vy & 
+            (%Hvx & %Hvy)))])" "close".
+      { iMod (Seen_valid with "[] [$Seen $z_hz']") as "(z_hz' & %abs)";
+          [solve_ndisj|iApply SI_GlobalInv|by apply suffix_nil_inv in abs].
+      }
+      iModIntro.
+      iExists {[ "x" := hx'; "y" := hy'; "z" := hz' ]}.
+      iSplit; first by rewrite !dom_insert_L.
+      iSplitL "x_hx' y_hy' z_hz'";
+        first by repeat (iApply big_sepM_insert; first done; iFrame).
+      iSplitR.
+      {
+        iExists hx', hy', hz', vx, vy.
+        iFrame "%".
+        by rewrite (lookup_insert_ne _ _ "y").
+      }
+      iSplitR; first done.
+      iIntros "!>(mem & _)".
+      iMod ("close" with "[mem]") as "_"; last done.
+      iNext.
+      iExists hx', hy', hz'.
+      iPoseProof (big_sepM_insert with "mem") as "(x_hx' & mem)"; first done.
+      iPoseProof (big_sepM_insert with "mem") as "(y_hy' & mem)"; first done.
+      iPoseProof (big_sepM_insert with "mem") as "(z_hz' & _)"; first done.
+      iFrame.
+      iRight.
+      iSplit; first done.
+      by iExists vx, vy.
+    }
+    {
+      iModIntro.
+      iInv "inv" as ">(%hx' & %hy' & %hz' & x_hx' & y_hy' & z_hz' &
+          %Hinv)" "close".
+      iModIntro.
+      iExists {[ "x" := hx'; "y" := hy'; "z" := hz' ]}.
+      iSplit; first by rewrite !dom_insert_L.
+      iSplitL "x_hx' y_hy' z_hz'";
+        first by repeat (iApply big_sepM_insert; first done; iFrame).
+      iIntros "!>mem".
+      iMod ("close" with "[mem]") as "_"; last done.
+      iNext.
+      iExists hx', hy', hz'.
+      iPoseProof (big_sepM_insert with "mem") as "(x_hx' & mem)"; first done.
+      iPoseProof (big_sepM_insert with "mem") as "(y_hy' & mem)"; first done.
+      iPoseProof (big_sepM_insert with "mem") as "(z_hz' & _)"; first done.
+      iFrame "∗ %".
+    }
+    {
+      iIntros (v' Ψ) "!>_ HΨ".
+      wp_pures.
+      wp_op; first apply bin_op_eval_eq_val.
+      iApply "HΨ".
+      by rewrite bool_decide_spec.
+    }
+    rewrite !dom_insert_L.
+    iClear (hx hy hz) "".
+    iIntros (m) "(%dom_m & (%hx & %hy & %hz & %vx & %vy & %m_x & %m_y & %m_z &
+          %hz_not_empty & %hx_vx & %hy_vy & %Hvx & %Hvy) & Active & cache & Seen)".
+    wp_pures.
+    iPoseProof (big_sepM_delete _ _ _ _ m_x with "cache") as
+        "((x_hx & x_upd) & cache)".
+    iPoseProof (big_sepM_delete _ _ "y" hy with "cache") as
+        "((y_hy & y_upd) & cache)"; first by rewrite lookup_delete_ne.
+    iPoseProof (big_sepM_delete _ _ "z" hz with "cache") as
+        "((z_hz & z_upd) & _)"; first by rewrite !lookup_delete_ne.
+    iPoseProof (big_sepM_lookup _ _ _ _ m_z with "Seen") as "#Seen_z".
+    wp_apply (SI_read_spec with "[] y_hy"); first set_solver.
+    iIntros "y_hy".
+    rewrite hx_vx hy_vy.
+    destruct Hvy as [-> | ->].
+    {
+      wp_pures.
+      wp_apply (SI_write_spec $! _ _ _ _ (SerVal #(-1)) with
+          "[] [$x_hx $x_upd]"); first set_solver.
+      iIntros "(x_1 & x_upd)".
+      wp_pures.
+      wp_apply (commitU_spec _ _ (⊤ ∖ ↑client_inv_name)); first solve_ndisj.
+      iInv "inv" as ">(%hx' & %hy' & %hz' & x_hx' & y_hy' & z_hz' &
+          [(_ & _ & ->)|(%hz'_not_empty & %vx' & %vy' & %hx'_vx' & 
+            %hy'_vy' & %Hvx' & %Hvy')])" "close".
+      {
+        iMod (Seen_valid $! SI_GlobalInv with "[$Seen_z $z_hz']") as
+            "(z_hz' & %abs)"; first solve_ndisj.
+        apply suffix_nil_inv in abs.
+        rewrite abs in hz_not_empty.
+        by apply elem_of_nil in hz_not_empty.
+      }
+      iModIntro.
+      iExists {[ "x" := hx'; "y" := hy'; "z" := hz' ]}, m,
+              {[ "x" := (Some #(-1), true); "y" := (Some #1, false);
+                  "z" := (hist_val hz, false) ]}.
+      iFrame.
+      iSplitL "x_1 x_hx' x_upd y_hy y_hy' y_upd z_hz z_hz' z_upd".
+      {
+        rewrite !dom_insert_L dom_m !dom_empty_L.
+        do 2 (iSplit; first done).
+        by iSplitL "x_hx' y_hy' z_hz'";
+            repeat (iApply big_sepM_insert; first done; iFrame).
+      }
+      iIntros "!>(_ & [(_ & mem)|(_ & mem)])".
+      {
+        iMod ("close" with "[mem]") as "_"; last by iApply "HΦ".
+        iPoseProof (big_sepM2_insert with "mem") as "((x_hx' & _) & mem)";
+          [done..|].
+        iPoseProof (big_sepM2_insert with "mem") as "((y_hy' & _) & mem)";
+          [done..|].
+        iPoseProof (big_sepM2_insert with "mem") as "((z_hz' & _) & _)";
+          [done..|].
+        have -> : commit_event (hist_val hz, false) hz' = hz'
+              by case: (hist_val hz).
+        iNext.
+        iExists (#(-1) :: hx'), hy', hz'.
+        iFrame.
+        iPureIntro.
+        right.
+        split; first done.
+        exists #(-1), vy'.
+        do 2 (split; first done).
+        by split; first right.
+      }
+      iMod ("close" with "[mem]") as "_"; last by iApply "HΦ".
+      iPoseProof (big_sepM_insert with "mem") as "((x_hx' & _) & mem)";
+          first done.
+      iPoseProof (big_sepM_insert with "mem") as "((y_hy' & _) & mem)";
+          first done.
+      iPoseProof (big_sepM_insert with "mem") as "((z_hz' & _) & _)";
+          first done.
+      iNext.
+      iExists _, _, _.
+      iFrame.
+      iPureIntro.
+      right.
+      split; first done.
+      by exists vx', vy'.
+    }
+    wp_pures.
+    wp_apply (commitU_spec _ _ (⊤ ∖ ↑client_inv_name)); first solve_ndisj.
+    iInv "inv" as ">(%hx' & %hy' & %hz' & x_hx' & y_hy' & z_hz' &
+          %Hinv)" "close".
+    iModIntro.
+    iExists {[ "x" := hx'; "y" := hy'; "z" := hz' ]}, m,
+            {[ "x" := (Some vx, false); "y" := (Some #(-1), false);
+                "z" := (hist_val hz, false) ]}.
+    iFrame.
+    iSplitL "x_upd x_hx x_hx' y_upd y_hy y_hy' z_upd z_hz z_hz'".
+    {
+      rewrite !dom_insert_L dom_m !dom_empty_L.
+      do 2 (iSplit; first done).
+      by iSplitL "x_hx' y_hy' z_hz'";
+          repeat (iApply big_sepM_insert; first done; iFrame).
+    }
+    iIntros "!>(_ & [(_ & mem)|(_ & mem)])".
+    {
+      iMod ("close" with "[mem]") as "_"; last by iApply "HΦ".
+      iPoseProof (big_sepM2_insert with "mem") as "((x_hx' & _) & mem)";
+        [done..|].
+      iPoseProof (big_sepM2_insert with "mem") as "((y_hy' & _) & mem)";
+        [done..|].
+      iPoseProof (big_sepM2_insert with "mem") as "((z_hz' & _) & _)";
+        [done..|].
+      have -> : commit_event (hist_val hz, false) hz' = hz'
+            by case: (hist_val hz).
+      iNext.
+      iExists hx', hy', hz'.
+      by iFrame.
+    }
+    iMod ("close" with "[mem]") as "_"; last by iApply "HΦ".
+    iPoseProof (big_sepM_insert with "mem") as "((x_hx' & _) & mem)";
+      [done..|].
+    iPoseProof (big_sepM_insert with "mem") as "((y_hy' & _) & mem)";
+      [done..|].
+    iPoseProof (big_sepM_insert with "mem") as "((z_hz' & _) & _)";
+      [done..|].
+    iNext.
+    iExists _, _, _.
+    by iFrame.
+  Qed.
+
+  Lemma transaction4_spec :
+    ∀ cst sa,
+    client_inv -∗
+    {{{ ConnectionState cst CanStart }}}
+      transaction4 cst @[ip_of_address sa]
+    {{{ RET #(); True }}}.
+  Proof.
+    iIntros (cst sa) "#inv %Φ !>CanStart HΦ".
+    rewrite/transaction4.
+    wp_pures.
+    wp_apply (SI_start_spec $! _ _ (⊤ ∖ ↑client_inv_name)); first solve_ndisj.
+    iInv "inv" as ">(%hx & %hy & %hz & x_hx & y_hy & z_hz & init)" "close".
+    iModIntro.
+    iExists {[ "x" := hx; "y" := hy; "z" := hz ]}.
+    iFrame.
+    iSplitL "x_hx y_hy z_hz";
+      first by repeat (iApply big_sepM_insert; first done; iFrame).
+    iIntros "!>(Active & mem & cache & Seen)".
+    iMod ("close" with "[mem init]") as "_".
+    {
+      iNext.
+      iExists hx, hy, hz.
+      iPoseProof (big_sepM_insert with "mem") as "(x_hx & mem)"; first done.
+      iPoseProof (big_sepM_insert with "mem") as "(y_hy & mem)"; first done.
+      iPoseProof (big_sepM_insert with "mem") as "(z_hz & _)"; first done.
+      iFrame.
+    }
+    iModIntro.
+    wp_pures.
+    wp_apply (simplified_wait_on_keyT_spec _ _ #1 _ _ _ (⊤ ∖ ↑client_inv_name)
+        (λ m, ∃ hx hy hz vx vy, ⌜m !! "x" = Some hx⌝ ∗ ⌜m !! "y" = Some hy⌝ ∗
+          ⌜m !! "z" = Some hz⌝ ∗ ⌜#1 ∈ hz⌝ ∗
+          ⌜hist_val hx = Some vx⌝ ∗ ⌜hist_val hy = Some vy⌝ ∗
+          (⌜vx = #1⌝ ∨ ⌜vx = #(-1)⌝) ∗ (⌜vy = #1⌝ ∨ ⌜vy = #(-1)⌝))%I
+          emp emp with
+          "[] [] [] [] [] [] [$Active $cache $Seen]"); first solve_ndisj.
+    1, 2 : rewrite !dom_insert_L; iPureIntro; set_solver.
+    {
+      iIntros "!>%h (#Seen & _)".
+      iInv "inv" as ">(%hx' & %hy' & %hz' & x_hx' & y_hy' & z_hz' &
+          [(_ & _ & ->)|(%hz'_1 & (%vx & %vy & %hx'_vx & %hy'_vy & 
+            (%Hvx & %Hvy)))])" "close".
+      { iMod (Seen_valid with "[] [$Seen $z_hz']") as "(z_hz' & %abs)";
+          [solve_ndisj|iApply SI_GlobalInv|by apply suffix_nil_inv in abs].
+      }
+      iModIntro.
+      iExists {[ "x" := hx'; "y" := hy'; "z" := hz' ]}.
+      iSplit; first by rewrite !dom_insert_L.
+      iSplitL "x_hx' y_hy' z_hz'";
+        first by repeat (iApply big_sepM_insert; first done; iFrame).
+      iSplitR.
+      {
+        iExists hx', hy', hz', vx, vy.
+        iFrame "%".
+        by rewrite (lookup_insert_ne _ _ "y").
+      }
+      iSplitR; first done.
+      iIntros "!>(mem & _)".
+      iMod ("close" with "[mem]") as "_"; last done.
+      iNext.
+      iExists hx', hy', hz'.
+      iPoseProof (big_sepM_insert with "mem") as "(x_hx' & mem)"; first done.
+      iPoseProof (big_sepM_insert with "mem") as "(y_hy' & mem)"; first done.
+      iPoseProof (big_sepM_insert with "mem") as "(z_hz' & _)"; first done.
+      iFrame.
+      iRight.
+      iSplit; first done.
+      by iExists vx, vy.
+    }
+    {
+      iModIntro.
+      iInv "inv" as ">(%hx' & %hy' & %hz' & x_hx' & y_hy' & z_hz' &
+          %Hinv)" "close".
+      iModIntro.
+      iExists {[ "x" := hx'; "y" := hy'; "z" := hz' ]}.
+      iSplit; first by rewrite !dom_insert_L.
+      iSplitL "x_hx' y_hy' z_hz'";
+        first by repeat (iApply big_sepM_insert; first done; iFrame).
+      iIntros "!>mem".
+      iMod ("close" with "[mem]") as "_"; last done.
+      iNext.
+      iExists hx', hy', hz'.
+      iPoseProof (big_sepM_insert with "mem") as "(x_hx' & mem)"; first done.
+      iPoseProof (big_sepM_insert with "mem") as "(y_hy' & mem)"; first done.
+      iPoseProof (big_sepM_insert with "mem") as "(z_hz' & _)"; first done.
+      iFrame "∗ %".
+    }
+    {
+      iIntros (v' Ψ) "!>_ HΨ".
+      wp_pures.
+      wp_op; first apply bin_op_eval_eq_val.
+      iApply "HΨ".
+      by rewrite bool_decide_spec.
+    }
+    rewrite !dom_insert_L.
+    iClear (hx hy hz) "".
+    iIntros (m) "(%dom_m & (%hx & %hy & %hz & %vx & %vy & %m_x & %m_y & %m_z &
+          %hz_not_empty & %hx_vx & %hy_vy & %Hvx & %Hvy) & Active & cache & Seen)".
+    wp_pures.
+    iPoseProof (big_sepM_delete _ _ _ _ m_x with "cache") as
+        "((x_hx & x_upd) & cache)".
+    iPoseProof (big_sepM_delete _ _ "y" hy with "cache") as
+        "((y_hy & y_upd) & cache)"; first by rewrite lookup_delete_ne.
+    iPoseProof (big_sepM_delete _ _ "z" hz with "cache") as
+        "((z_hz & z_upd) & _)"; first by rewrite !lookup_delete_ne.
+    iPoseProof (big_sepM_lookup _ _ _ _ m_z with "Seen") as "#Seen_z".
+    wp_apply (SI_read_spec with "[] x_hx"); first set_solver.
+    iIntros "x_hx".
+    wp_apply wp_unSOME; first by rewrite hx_vx.
+    iIntros "_".
+    wp_pures.
+    wp_apply (SI_read_spec with "[] y_hy"); first set_solver.
+    iIntros "y_hy".
+    wp_apply wp_unSOME; first by rewrite hy_vy.
+    iIntros "_".
+    wp_pures.
+    iAssert (∀ a b : Z, ⌜vx = #a⌝ ∗ ⌜vy = #b⌝ ∗
+        ⌜(a + b ≠ -2)%Z → (0 ≤ a + b)%Z⌝ -∗
+        WP let: "r" := vx + vy in
+        assert: (if: "r" = #(-2) then #true else #0 ≤ "r") ;; 
+        util_code.commitU cst @[ip_of_address sa] {{ v, Φ v }})%I with 
+       "[HΦ Active x_upd y_upd z_upd x_hx y_hy z_hz]" as "finish".
+    {
+      iIntros (a b) "(-> & -> & %Hab)".
+      wp_pures.
+      rewrite /assert.
+      wp_pures.
+      case eq: (bool_decide (a + b = -2)%Z).
+      {
+        wp_pures.
+        wp_apply (commitU_spec _ _ (⊤ ∖ ↑client_inv_name)); first solve_ndisj.
+        iInv "inv" as ">(%hx' & %hy' & %hz' & x_hx' & y_hy' & z_hz' & %Hinv)"
+                          "close".
+        iModIntro.
+        iExists {[ "x" := hx'; "y" := hy'; "z" := hz' ]}, _,
+                {[ "x" := (hist_val hx, false); "y" := (hist_val hy, false);
+                   "z" := (hist_val hz, false) ]}.
+        iFrame.
+        iSplitL "x_upd x_hx x_hx' y_upd y_hy y_hy' z_upd z_hz z_hz'".
+        {
+          rewrite !dom_insert_L dom_m !dom_empty_L.
+          do 2 (iSplit; first done).
+          by iSplitL "x_hx' y_hy' z_hz'";
+             repeat (iApply big_sepM_insert; first done; iFrame).
+        }
+        iIntros "!>(_ & [(_ & mem)|(_ & mem)])".
+        {
+          iMod ("close" with "[mem]") as "_"; last by iApply "HΦ".
+          iPoseProof (big_sepM2_insert with "mem") as "((x_hx' & _) & mem)";
+            [done..|].
+          iPoseProof (big_sepM2_insert with "mem") as "((y_hy' & _) & mem)";
+            [done..|].
+          iPoseProof (big_sepM2_insert with "mem") as "((z_hz' & _) & _)";
+            [done..|].
+          have -> : commit_event (hist_val hx, false) hx' = hx'
+                by case: (hist_val hx).
+          have -> : commit_event (hist_val hy, false) hy' = hy'
+                by case: (hist_val hy).
+          have -> : commit_event (hist_val hz, false) hz' = hz'
+                by case: (hist_val hz).
+          iNext.
+          iExists hx', hy', hz'.
+          by iFrame.
+        }
+        iMod ("close" with "[mem]") as "_"; last by iApply "HΦ".
+        iPoseProof (big_sepM_insert with "mem") as "((x_hx' & _) & mem)";
+          [done..|].
+        iPoseProof (big_sepM_insert with "mem") as "((y_hy' & _) & mem)";
+          [done..|].
+        iPoseProof (big_sepM_insert with "mem") as "((z_hz' & _) & _)";
+          [done..|].
+        iNext.
+        iExists _, _, _.
+        by iFrame.
+      }
+      wp_pures.
+      apply bool_decide_eq_false in eq.
+      rewrite bool_decide_true; last by apply Hab.
+      wp_pures.
+      wp_apply (commitU_spec _ _ (⊤ ∖ ↑client_inv_name)); first solve_ndisj.
+      iInv "inv" as ">(%hx' & %hy' & %hz' & x_hx' & y_hy' & z_hz' & %Hinv)"
+                        "close".
+      iModIntro.
+      iExists {[ "x" := hx'; "y" := hy'; "z" := hz' ]}, _,
+              {[ "x" := (hist_val hx, false); "y" := (hist_val hy, false);
+                 "z" := (hist_val hz, false) ]}.
+      iFrame.
+      iSplitL "x_upd x_hx x_hx' y_upd y_hy y_hy' z_upd z_hz z_hz'".
+      {
+        rewrite !dom_insert_L dom_m !dom_empty_L.
+        do 2 (iSplit; first done).
+        by iSplitL "x_hx' y_hy' z_hz'";
+           repeat (iApply big_sepM_insert; first done; iFrame).
+      }
+      iIntros "!>(_ & [(_ & mem)|(_ & mem)])".
+      {
+        iMod ("close" with "[mem]") as "_"; last by iApply "HΦ".
+        iPoseProof (big_sepM2_insert with "mem") as "((x_hx' & _) & mem)";
+          [done..|].
+        iPoseProof (big_sepM2_insert with "mem") as "((y_hy' & _) & mem)";
+          [done..|].
+        iPoseProof (big_sepM2_insert with "mem") as "((z_hz' & _) & _)";
+          [done..|].
+        have -> : commit_event (hist_val hx, false) hx' = hx'
+              by case: (hist_val hx).
+        have -> : commit_event (hist_val hy, false) hy' = hy'
+              by case: (hist_val hy).
+        have -> : commit_event (hist_val hz, false) hz' = hz'
+              by case: (hist_val hz).
+        iNext.
+        iExists hx', hy', hz'.
+        by iFrame.
+      }
+      iMod ("close" with "[mem]") as "_"; last by iApply "HΦ".
+      iPoseProof (big_sepM_insert with "mem") as "((x_hx' & _) & mem)";
+        [done..|].
+      iPoseProof (big_sepM_insert with "mem") as "((y_hy' & _) & mem)";
+        [done..|].
+      iPoseProof (big_sepM_insert with "mem") as "((z_hz' & _) & _)";
+        [done..|].
+      iNext.
+      iExists _, _, _.
+      by iFrame.
+    }
+    case: Hvx=>[->|->]; case: Hvy=>[->|->]; iApply "finish";
+        do 2 (iSplit; first done); iPureIntro; lia.
+  Qed.
+
+  Lemma transaction1_client_spec :
+    ∀ sa,
+    client_inv -∗
+    {{{
+      sa ⤳ (∅, ∅) ∗
+      unallocated {[sa]} ∗
+      free_ports (ip_of_address sa) {[port_of_address sa]} ∗
+      KVS_address ⤇ KVS_si
+    }}}
+      transaction1_client $sa $KVS_address @[ip_of_address sa]
+    {{{ RET #(); True }}}.
+  Proof.
+    iIntros (sa) "#inv %Φ !>(∅ & unalloc & free & #KVS_si) HΦ".
+    rewrite/transaction1_client.
+    wp_pures.
+    wp_apply (SI_init_client_proxy_spec with "[$]").
+    iIntros (cst) "CanStart".
+    wp_pures.
+    by wp_apply (transaction1_spec with "inv [$]").
+  Qed.
+
+  Lemma transaction2_client_spec :
+    ∀ sa,
+    client_inv -∗
+    {{{
+      sa ⤳ (∅, ∅) ∗
+      unallocated {[sa]} ∗
+      free_ports (ip_of_address sa) {[port_of_address sa]} ∗
+      KVS_address ⤇ KVS_si
+    }}}
+      transaction2_client $sa $KVS_address @[ip_of_address sa]
+    {{{ RET #(); True }}}.
+  Proof.
+    iIntros (sa) "#inv %Φ !>(∅ & unalloc & free & #KVS_si) HΦ".
+    rewrite/transaction2_client.
+    wp_pures.
+    wp_apply (SI_init_client_proxy_spec with "[$]").
+    iIntros (cst) "CanStart".
+    wp_pures.
+    by wp_apply (transaction2_spec with "inv [$]").
+  Qed.
+
+  Lemma transaction3_client_spec :
+    ∀ sa,
+    client_inv -∗
+    {{{
+      sa ⤳ (∅, ∅) ∗
+      unallocated {[sa]} ∗
+      free_ports (ip_of_address sa) {[port_of_address sa]} ∗
+      KVS_address ⤇ KVS_si
+    }}}
+      transaction3_client $sa $KVS_address @[ip_of_address sa]
+    {{{ RET #(); True }}}.
+  Proof.
+    iIntros (sa) "#inv %Φ !>(∅ & unalloc & free & #KVS_si) HΦ".
+    rewrite/transaction3_client.
+    wp_pures.
+    wp_apply (SI_init_client_proxy_spec with "[$]").
+    iIntros (cst) "CanStart".
+    wp_pures.
+    by wp_apply (transaction3_spec with "inv [$]").
+  Qed.
+
+  Lemma transaction4_client_spec :
+    ∀ sa,
+    client_inv -∗
+    {{{
+      sa ⤳ (∅, ∅) ∗
+      unallocated {[sa]} ∗
+      free_ports (ip_of_address sa) {[port_of_address sa]} ∗
+      KVS_address ⤇ KVS_si
+    }}}
+      transaction4_client $sa $KVS_address @[ip_of_address sa]
+    {{{ RET #(); True }}}.
+  Proof.
+    iIntros (sa) "#inv %Φ !>(∅ & unalloc & free & #KVS_si) HΦ".
+    rewrite/transaction4_client.
+    wp_pures.
+    wp_apply (SI_init_client_proxy_spec with "[$]").
+    iIntros (cst) "CanStart".
+    wp_pures.
+    by wp_apply (transaction4_spec with "inv [$]").
+  Qed.
+
+  Lemma server_spec :
+    {{{ KVS_Init
+      ∗ KVS_address ⤳ (∅, ∅)
+      ∗ free_ports (ip_of_address KVS_address) {[port_of_address KVS_address]}
+      ∗ KVS_address ⤇ KVS_si }}}
+    server #KVS_address @[ip_of_address KVS_address]
+    {{{ RET #(); True }}}.
+  Proof.
+    iIntros (Φ) "(? & ? & ? & ?) HΦ".
+    rewrite /server. wp_pures.
+    by wp_apply (SI_init_kvs_spec with "[$]").
+  Qed.
+
+End proofs.
+
+Section proof_runner.
+
+Context `{!anerisG Mdl Σ, !SI_init, !KVSG Σ}.
+
+  Definition example_runner : expr :=
+    let: "serveraddr" := MakeAddress #"0.0.0.0" #80 in
+    let: "client1addr" := MakeAddress #"0.0.0.1" #80 in
+    let: "client2addr" := MakeAddress #"0.0.0.2" #80 in
+    let: "client3addr" := MakeAddress #"0.0.0.3" #80 in
+    let: "client4addr" := MakeAddress #"0.0.0.4" #80 in
+    Start "0.0.0.0" (server "serveraddr") ;;
+    Start "0.0.0.1" (transaction1_client "client1addr" "serveraddr") ;;
+    Start "0.0.0.2" (transaction2_client "client2addr" "serveraddr") ;;
+    Start "0.0.0.3" (transaction3_client "client3addr" "serveraddr") ;;
+    Start "0.0.0.4" (transaction4_client "client4addr" "serveraddr").
+
+  Lemma example_runner_spec :
+    {{{ server_addr ⤳ (∅, ∅)
+      ∗ client_1_addr ⤳ (∅, ∅)
+      ∗ client_2_addr ⤳ (∅, ∅)
+      ∗ client_3_addr ⤳ (∅, ∅)
+      ∗ client_4_addr ⤳ (∅, ∅)
+      ∗ unallocated {[server_addr]}
+      ∗ unallocated {[client_1_addr]}
+      ∗ unallocated {[client_2_addr]}
+      ∗ unallocated {[client_3_addr]}
+      ∗ unallocated {[client_4_addr]}
+      ∗ free_ip (ip_of_address server_addr)
+      ∗ free_ip (ip_of_address client_1_addr)
+      ∗ free_ip (ip_of_address client_2_addr)
+      ∗ free_ip (ip_of_address client_3_addr)
+      ∗ free_ip (ip_of_address client_4_addr)
+     }}}
+      example_runner @["system"]
+    {{{ RET #(); True }}}.
+  Proof.
+    iMod SI_init_module as (SI_res SI_client_toolbox) "(mem & KVS_Init)".
+    iPoseProof (big_sepS_delete _ _ "x" with "mem") as "(mem_x & mem)";
+      first done.
+    iPoseProof (big_sepS_delete _ _ "y" with "mem") as "(mem_y & mem)";
+      first done.
+    iPoseProof (big_sepS_delete _ _ "z" with "mem") as "(mem_z & _)";
+      first done.
+    iMod (inv_alloc client_inv_name _ client_inv_def with "[mem_x mem_y mem_z]")
+      as "#inv".
+    { iNext. iExists _, _, _. iFrame. by iLeft. }
+    iIntros (Φ) "(srv_∅ & clt1_∅ & clt2_∅ & clt3_∅ & clt4_∅ & srv_unalloc &
+      clt1_unalloc & clt2_unalloc & clt3_unalloc & clt4_unalloc &
+      ? & ? & ? & ? & ?) HΦ".
+    rewrite /example_runner.
+    wp_pures.
+    wp_apply (aneris_wp_socket_interp_alloc_singleton KVS_si with "srv_unalloc").
+    iIntros "#KVS_si".
+    wp_apply (aneris_wp_start {[80%positive]}).
+    iFrame.
+    iSplitR "srv_∅ KVS_Init"; last first.
+    {
+      iIntros "!>Hports".
+      by wp_apply (server_spec with "[$]").
+    }
+    iNext.
+    wp_pures.
+    wp_apply (aneris_wp_start {[80%positive]}).
+    iFrame.
+    iSplitR "clt1_∅ clt1_unalloc"; last first.
+    {
+      iIntros "!>Hports".
+      by wp_apply (transaction1_client_spec client_1_addr with "inv [$]").
+    }
+    iNext.
+    wp_pures.
+    wp_apply (aneris_wp_start {[80%positive]}).
+    iFrame.
+    iSplitR "clt2_∅ clt2_unalloc"; last first.
+    {
+      iIntros "!>Hports".
+      by wp_apply (transaction2_client_spec client_2_addr with "inv [$]").
+    }
+    iNext.
+    wp_pures.
+    wp_apply (aneris_wp_start {[80%positive]}).
+    iFrame.
+    iSplitR "clt3_∅ clt3_unalloc"; last first.
+    {
+      iIntros "!>Hports".
+      by wp_apply (transaction3_client_spec client_3_addr with "inv [$]").
+    }
+    iNext.
+    wp_pures.
+    wp_apply (aneris_wp_start {[80%positive]}).
+    iFrame.
+    iSplitR "clt4_∅ clt4_unalloc"; last first.
+    {
+      iIntros "!>Hports".
+      by wp_apply (transaction4_client_spec client_4_addr with "inv [$]").
+    }
+    by iApply "HΦ".
+  Qed.
+
+End proof_runner.
+
+Definition unit_model := model _ (λ _ _, False) ().
+Lemma unit_model_rel_finitary : aneris_model_rel_finitary unit_model.
+Proof. intros ?. apply finite_smaller_card_nat. apply _. Qed.
+
+Definition ips : gset string :=
+  {[ ip_of_address server_addr ; ip_of_address client_1_addr
+  ; ip_of_address client_2_addr ; ip_of_address client_3_addr
+  ; ip_of_address client_4_addr]}.
+
+Definition sa_dom : gset socket_address :=
+  {[ server_addr ; client_1_addr; client_2_addr; client_3_addr; client_4_addr ]}.
+
+Definition init_state :=
+  {|
+    state_heaps := {["system" := ∅ ]};
+    state_sockets := {["system" := ∅ ]};
+    state_ms := ∅;
+  |}.
+
+Theorem runner_safe :
+  aneris_adequate example_runner "system" init_state (λ _, True).
+Proof.
+  set (Σ := #[anerisΣ unit_model; KVSΣ]).
+  apply (@adequacy Σ unit_model _ _ ips sa_dom ∅ ∅ ∅); 
+  [apply unit_model_rel_finitary | |set_solver..].
+  iIntros (dinvG). iIntros "!> Hunallocated Hhist Hfrag Hips Hlbl _ _ _ _".
+  iApply (example_runner_spec with "[Hunallocated Hhist Hfrag Hips Hlbl]" ).
+  2 : { iModIntro. done. }
+  do 4 (iDestruct (unallocated_split with "Hunallocated") as "[Hunallocated ?]";
+  [set_solver|]). iFrame.
+  do 4 (rewrite big_sepS_union; [|set_solver];
+  rewrite !big_sepS_singleton;
+  iDestruct "Hhist" as "[Hhist ?]"; iFrame).
+  do 4 (rewrite big_sepS_union; [|set_solver];
+  rewrite !big_sepS_singleton;
+  iDestruct "Hips" as "[Hips ?]"; iFrame).
+Qed.
