aneris/examples/snapshot_isolation/examples/sequential_writes/sequential_writes_proof.v
@@ -1,0 +1,321 @@
+From aneris.aneris_lang Require Import network resources proofmode.
+From aneris.aneris_lang.lib Require Import
+     list_proof inject lock_proof.
+From aneris.aneris_lang.lib.serialization
+     Require Import serialization_proof.
+From aneris.aneris_lang.program_logic Require Import lightweight_atomic.
+From aneris.examples.snapshot_isolation.specs
+     Require Import user_params resources specs.
+From aneris.aneris_lang Require Import tactics proofmode adequacy.
+From trillium.prelude Require Import finitary.
+From aneris.aneris_lang.program_logic Require Import
+     aneris_weakestpre aneris_adequacy aneris_lifting.
+From iris.base_logic.lib Require Import invariants.
+From aneris.examples.snapshot_isolation.examples.sequential_writes 
+  Require Import sequential_writes_code.
+Import ser_inj.
+From aneris.examples.snapshot_isolation.instantiation
+     Require Import snapshot_isolation_api_implementation.
+From aneris.examples.snapshot_isolation.util Require Import util_proof.
+From iris.algebra Require Import excl.
+From aneris.examples.snapshot_isolation.examples Require Import proof_resources.
+
+Definition server_addr := SocketAddressInet "0.0.0.0" 80.
+Definition client_1_addr := SocketAddressInet "0.0.0.1" 80.
+Definition client_2_addr := SocketAddressInet "0.0.0.2" 80.
+
+Instance params : User_params :=
+{| KVS_address := server_addr;
+  KVS_keys := {["x"]};
+  KVS_InvName := nroot .@ "siinv";
+  KVS_serialization := int_serialization;
+  KVS_ser_inj := int_ser_is_ser_injective;
+  KVS_ser_inj_alt := int_ser_is_ser_injective_alt
+|}.
+
+Definition client_inv_name := nroot.@"clinv".
+
+Section proofs.
+
+Context `{!anerisG Mdl Σ, !SI_resources Mdl Σ, !SI_client_toolbox, !KVSG Σ}.
+
+  Definition client_inv (γF1 γF2 : gname): iProp Σ :=
+    ∃ hx, "x" ↦ₖ hx ∗
+    ((⌜hx = [(#2);(#1)]⌝ ∗ token γF1 ∗ token γF2)
+    ∨ (⌜hx = [(#1)]⌝ ∗ token γF1)
+    ∨ (⌜hx = []⌝)).
+
+  Lemma server_spec ip port :
+    ip = ip_of_address KVS_address →
+    port = port_of_address KVS_address →
+    {{{ KVS_Init
+      ∗ KVS_address ⤳ (∅, ∅)
+      ∗ free_ports ip {[port]}
+      ∗ KVS_address ⤇ KVS_si }}}
+    server #KVS_address @[ip]
+    {{{ RET #(); True }}}.
+  Proof.
+    iIntros (Hip Hports Φ) "(? & ? & ? & ?) HΦ".
+    rewrite /server. wp_pures. rewrite Hip Hports.
+    by wp_apply (SI_init_kvs_spec with "[$]").
+  Qed.
+
+  Lemma client_1_spec ip port γF1 γF2:
+  ip = ip_of_address client_1_addr →
+  port = port_of_address client_1_addr →
+  {{{ inv client_inv_name (client_inv γF1 γF2)
+    ∗ token γF1
+    ∗ client_1_addr ⤳ (∅, ∅)
+    ∗ unallocated {[client_1_addr]}
+    ∗ free_ports ip {[port]}
+    ∗ KVS_address ⤇ KVS_si }}}
+    transaction1_client $client_1_addr $KVS_address @[ip]
+  {{{ v, RET v; True }}}.
+  Proof.
+    iIntros (Hip Hports Φ) "(#Hinv & Htok & Hmsghis & Hunalloc
+    & Hports & Hprot) HΦ".
+    rewrite /transaction1_client. wp_pures. rewrite Hip Hports.
+    wp_apply (SI_init_client_proxy_spec with "[$Hunalloc $Hprot $Hmsghis $Hports]").
+    iIntros (rpc) "Hcstate". wp_pures. rewrite /transaction1. wp_pures.
+    wp_apply (SI_start_spec $! rpc client_1_addr (⊤ ∖ ↑client_inv_name)); try solve_ndisj.
+    iInv (client_inv_name) as ">[%hx [Hkx [(_ & Htok' & _) | [(_ & Htok') | %Heq]]]]" "HClose";
+    try iDestruct (token_exclusive with "Htok Htok'") as "[]".
+    iModIntro. iFrame.
+    iExists {["x" := hx]}.
+    rewrite !big_sepM_insert; try set_solver.
+    rewrite big_sepM_empty.
+    iSplitL "Hkx"; first iFrame.
+    iNext. iIntros "(Hcstate & [Hkx _] & [Hcx _] & _)".
+    iMod ("HClose" with "[Hkx]") as "_".
+    { iNext. iExists hx. iFrame. set_solver. }
+    iModIntro. wp_pures.
+    wp_apply (SI_write_spec $! _ _ _ _ (SerVal #1) with "[] [Hcx]"). 
+    set_solver. iFrame. iIntros "Hcx". wp_pures.
+    wp_apply (commitT_spec rpc client_1_addr (⊤ ∖ ↑client_inv_name));
+    try solve_ndisj.
+    iInv (client_inv_name) as ">[%hx' [Hkx [(_ & Htok' & _) | [(_ & Htok') | %Heq']]]]" "HClose";
+    try iDestruct (token_exclusive with "Htok Htok'") as "[]".
+    iModIntro.
+    iExists {["x" := hx']}, _, {["x" := (Some #1, true)]}.
+    rewrite Heq Heq'.
+    iFrame. iSplitL "Hcx Hkx". 
+      - iSplitR "Hcx Hkx"; try iSplitR "Hcx Hkx";
+        try iPureIntro; try set_solver.
+        rewrite !big_sepM_insert; try set_solver.
+        rewrite !big_sepM_empty. iFrame.
+        iPureIntro. set_solver.
+      - iNext. iIntros "[_ HBig]". 
+        iMod ("HClose" with "[HBig Htok]") as "_".
+            + iNext. iExists [(#1)]. 
+              rewrite !(big_sepM2_insert); try set_solver.
+              iDestruct "HBig" as "[[Hx _] _]".
+              iFrame. set_solver.
+            + iModIntro. by iApply "HΦ".
+  Qed.
+
+  Lemma client_2_spec ip port γF1 γF2:
+    ip = ip_of_address client_2_addr →
+    port = port_of_address client_2_addr →
+    {{{ inv client_inv_name (client_inv γF1 γF2)
+      ∗ token γF2
+      ∗ client_2_addr ⤳ (∅, ∅)
+      ∗ unallocated {[client_2_addr]}
+      ∗ free_ports ip {[port]}
+      ∗ KVS_address ⤇ KVS_si }}}
+      transaction2_client $client_2_addr $KVS_address @[ip]
+    {{{ v, RET v; True }}}.
+  Proof. 
+    iIntros (Hip Hports Φ) "(#Hinv & Htok & Hmsghis & Hunalloc
+    & Hports & Hprot) HΦ".
+    rewrite /transaction2_client. wp_pures. rewrite Hip Hports.
+    wp_apply (SI_init_client_proxy_spec with "[$Hunalloc $Hprot $Hmsghis $Hports]").
+    iIntros (rpc) "Hcstate". wp_pures. rewrite /transaction2. wp_pures.
+    wp_apply (SI_start_spec $! rpc client_2_addr (⊤ ∖ ↑client_inv_name)); try solve_ndisj.
+    iInv (client_inv_name) as ">[%hx [Hkx [(_ & _ & Htok') | Hrest]]]" "HClose";
+    try iDestruct (token_exclusive with "Htok Htok'") as "[]".
+    iModIntro. iFrame.
+    iExists {["x" := hx]}.
+    rewrite !big_sepM_insert; try set_solver.
+    rewrite big_sepM_empty.
+    iSplitL "Hkx"; first iFrame.
+    iNext. iIntros "(Hcstate & [Hkx _] & [Hcx _] & Hseen & _)".
+    iMod ("HClose" with "[Hkx Hrest]") as "_".
+    { iNext. iExists hx. iFrame. }
+    iModIntro. wp_pures.
+    wp_apply (simplified_wait_on_keyT_spec _ _ (#1) _ 
+      {["x":= hx]} _ (⊤ ∖ ↑client_inv_name) 
+      (λ m, ⌜m = {["x":=[(#1)]]}⌝ ∗ token γF2)%I (token γF2) (token γF1)
+      with "[] [] [] [] [] [] [Hcx Hcstate Hseen Htok] [HΦ]");
+    try solve_ndisj; try iPureIntro; try set_solver.
+      - iModIntro. iIntros (h) "(Hxseen & Htok)". 
+        iInv (client_inv_name) as ">[%hx' [Hkx [(_ & _ & Htok') | [(-> & Htok') | ->]]]]" "HClose".
+        + iDestruct (token_exclusive with "Htok Htok'") as "[]".
+        + iModIntro. iExists {["x":= [(#1)]]}.
+          iSplit. 
+          { iPureIntro. set_solver. }
+          iSplitL "Hkx".
+          { rewrite !big_sepM_insert; set_solver. }
+          iSplitL "Htok".
+          { by iFrame. }
+          iFrame. iIntros "!> [Hkx Htok]". 
+          iMod ("HClose" with "[Htok Hkx]") as "_"; try done.
+          iNext. iExists _. 
+          rewrite !(big_sepM_insert); try set_solver.
+          iDestruct "Hkx" as "[Hkx _]". iFrame.
+          iRight. iLeft. by iFrame.
+          + iDestruct (Seen_valid (⊤ ∖ ↑client_inv_name) with "[]") as "Hfalse"; 
+          [solve_ndisj|iApply SI_GlobalInv|].
+          iMod ("Hfalse" with "[$Hxseen $Hkx]") as "(Hkx & %Hfalse)".
+          destruct Hfalse as [? Hfalse].
+          by apply app_cons_not_nil in Hfalse.
+      - iModIntro. 
+        iInv (client_inv_name) as ">[%hx' [Hkx Hrest]]" "HClose".
+        iModIntro.
+        iExists {["x":= hx']}.
+        iSplit. 
+        { iPureIntro. set_solver. }
+        iSplitL "Hkx".
+        { rewrite !big_sepM_insert; set_solver. }
+        iIntros "!> Hkx". 
+        iMod ("HClose" with "[Hkx Hrest]") as "_"; try done.
+        iNext. iExists _. 
+        rewrite !(big_sepM_insert); try set_solver.
+        iDestruct "Hkx" as "[Hkx _]". iFrame.
+      - iIntros (v Φ') "!>Htrue HΦ".
+        wp_lam. wp_op.
+        apply bin_op_eval_eq_val.
+        case_bool_decide as Heq;
+        iApply "HΦ"; set_solver.
+      - rewrite !(big_sepM_insert); try set_solver.
+        rewrite !big_sepM_empty. iFrame.
+      - iNext. iIntros (ms) "(%Hdom & (-> & Htok) & Hcp & Hx & Hseen)".
+        wp_pures.
+        wp_apply (SI_write_spec $! _ _ _ _ (SerVal #2) with "[] [Hx]"). 
+        set_solver.
+        {
+          rewrite !big_sepM_insert; try set_solver.
+          rewrite big_sepM_empty. iDestruct "Hx" as "[[? ?] _]". iFrame.
+        }
+        iIntros "Hcx". wp_pures.
+        wp_apply (commitT_spec rpc client_2_addr (⊤ ∖ ↑client_inv_name));
+        try solve_ndisj.
+        iInv (client_inv_name) as ">[%hx' [Hkx [(_ & _ & Htok') | [(-> & Htok') | ->]]]]" "HClose".
+        + iDestruct (token_exclusive with "Htok Htok'") as "[]".
+        + iModIntro. iExists {["x" := [(#1)]]}, _, {["x" := (Some #2, true)]}.
+          iFrame. iSplitL "Hcx Hkx". 
+          * iSplitR "Hcx Hkx"; try iSplitR "Hcx Hkx";
+            try iPureIntro; try set_solver.
+            rewrite !big_sepM_insert; try set_solver.
+            rewrite !big_sepM_empty. iFrame.
+          * iNext. iIntros "[_ HBig]". 
+            iMod ("HClose" with "[HBig Htok Htok']") as "_".
+            -- iNext. iExists [(#2);(#1)]. 
+               rewrite !(big_sepM2_insert); try set_solver.
+               iDestruct "HBig" as "[[Hx _] _]".
+               iFrame. iLeft. by iFrame.
+            -- iModIntro. by iApply "HΦ".
+        + rewrite !big_sepM_insert; last set_solver.
+        iDestruct "Hseen" as "[Hseen _]". 
+        iDestruct (Seen_valid (⊤ ∖ ↑client_inv_name) with "[]") as "Hfalse"; 
+        [solve_ndisj|iApply SI_GlobalInv|].
+        iMod ("Hfalse" with "[$Hseen $Hkx]") as "(Kkx & %Hfalse)".
+        destruct Hfalse as [? Hfalse].
+        by apply app_cons_not_nil in Hfalse.
+  Qed.
+
+End proofs.
+
+Section proof_runner.
+
+Context `{!anerisG Mdl Σ, !SI_init, !KVSG Σ}.
+
+  Definition example_runner : expr :=
+    let: "serveraddr" := MakeAddress #"0.0.0.0" #80 in
+    let: "client1addr" := MakeAddress #"0.0.0.1" #80 in
+    let: "client2addr" := MakeAddress #"0.0.0.2" #80 in
+    Start "0.0.0.0" (server "serveraddr") ;;
+    Start "0.0.0.1" (transaction1_client "client1addr" "serveraddr") ;;
+    Start "0.0.0.2" (transaction2_client "client2addr" "serveraddr").
+
+  Lemma example_runner_spec :
+    {{{ server_addr ⤳ (∅, ∅)
+      ∗ client_1_addr ⤳ (∅, ∅)
+      ∗ client_2_addr ⤳ (∅, ∅)
+      ∗ unallocated {[server_addr]}
+      ∗ unallocated {[client_1_addr]}
+      ∗ unallocated {[client_2_addr]}
+      ∗ free_ip (ip_of_address server_addr)
+      ∗ free_ip (ip_of_address client_1_addr)
+      ∗ free_ip (ip_of_address client_2_addr) }}}
+      example_runner @["system"]
+    {{{ v, RET v; True }}}.
+  Proof.
+    iMod SI_init_module as (SI_res SI_specs) "(HKVSres & HVKSinit)".
+    iMod (own_alloc (Excl ())) as (γF1) "Hftk1"; first done.
+    iMod (own_alloc (Excl ())) as (γF2) "Hftk2"; first done.
+    iMod (inv_alloc client_inv_name ⊤ (client_inv γF1 γF2) with "[HKVSres]") as "#Hinv".
+    { iNext. iExists [].
+    iDestruct (big_sepS_delete _ _ "x" with "HKVSres") as "(Hx & HKVSres)";
+    first set_solver. iFrame. set_solver.
+    }
+    iIntros (Φ) "(Hsrvhist & Hcli1hist & Hcli2hist & Hsrvunalloc & Hcli1unalloc 
+    & Hcli2unalloc & ? & ? & ?) HΦ".
+    rewrite /example_runner.
+    wp_pures.
+    wp_apply (aneris_wp_socket_interp_alloc_singleton KVS_si with "Hsrvunalloc").
+    iIntros "#HKVS_si".
+    wp_apply (aneris_wp_start {[80%positive]}).
+    iFrame.
+    iSplitR "Hsrvhist HVKSinit".
+    - iModIntro. wp_pures.
+      wp_apply (aneris_wp_start {[80%positive : port]}).
+      iFrame.
+      iSplitR "Hcli1hist Hcli1unalloc Hftk1".
+      + iModIntro. wp_pures.
+        wp_apply (aneris_wp_start {[80%positive : port]}).
+        iFrame.
+        iSplitR "Hcli2hist Hcli2unalloc Hftk2".
+        * by iApply "HΦ". 
+        * iIntros "!> Hports". wp_apply (client_2_spec with "[$]"); try done. 
+      + iIntros "!> Hports". wp_apply (client_1_spec with "[$]"); try done. 
+    - iIntros "!> Hports". wp_apply (server_spec with "[$]"); done.
+  Qed.
+
+End proof_runner.
+
+Definition unit_model := model _ (λ _ _, False) ().
+Lemma unit_model_rel_finitary : aneris_model_rel_finitary unit_model.
+Proof. intros ?. apply finite_smaller_card_nat. apply _. Qed.
+
+Definition ips : gset string :=
+  {[ ip_of_address server_addr ; ip_of_address client_1_addr
+  ; ip_of_address client_2_addr ]}.
+
+Definition sa_dom : gset socket_address :=
+  {[ server_addr ; client_1_addr; client_2_addr ]}.
+
+Definition init_state :=
+  {|
+    state_heaps := {["system" := ∅ ]};
+    state_sockets := {["system" := ∅ ]};
+    state_ms := ∅;
+  |}.
+
+Theorem runner_safe :
+  aneris_adequate example_runner "system" init_state (λ _, True).
+Proof.
+  set (Σ := #[anerisΣ unit_model; KVSΣ]).
+  apply (@adequacy Σ unit_model _ _ ips sa_dom ∅ ∅ ∅);
+    [apply unit_model_rel_finitary| |set_solver..].
+  iIntros (dinvG). iIntros "!> Hunallocated Hhist Hfrag Hips Hlbl _ _ _ _".
+  iApply (example_runner_spec with "[Hunallocated Hhist Hfrag Hips Hlbl]" ).
+  2 : { iModIntro. done. }
+  do 2 (iDestruct (unallocated_split with "Hunallocated") as "[Hunallocated ?]";
+  [set_solver|]). iFrame.
+  do 2 (rewrite big_sepS_union; [|set_solver];
+  rewrite !big_sepS_singleton;
+  iDestruct "Hhist" as "[Hhist ?]"; iFrame).
+  do 2 (rewrite big_sepS_union; [|set_solver];
+  rewrite !big_sepS_singleton;
+  iDestruct "Hips" as "[Hips ?]"; iFrame).
+Qed.
