aneris/examples/snapshot_isolation/instantiation/snapshot_isolation_api_implementation.v
@@ -1,0 +1,22 @@
+From aneris.examples.snapshot_isolation
+     Require Import snapshot_isolation_code 
+                    snapshot_isolation_code_api.
+From aneris.aneris_lang Require Import resources.
+From aneris.examples.snapshot_isolation.specs Require Import user_params specs.
+
+Global Instance KVS_snapshot_isolation_api_implementation :
+        KVS_snapshot_isolation_api :=
+  {|
+    SI_init_server := init_server;
+    SI_start := start;
+    SI_read := read;
+    SI_write := write;
+    SI_commit := commit;
+    SI_run := run;
+    SI_init_client_proxy := init_client_proxy;
+  |}.
+
+Global Instance SI_init_instanciation `{!anerisG Mdl Σ, !User_params} :
+    SI_init.
+Proof.
+Admitted.
