aneris/examples/snapshot_isolation/proof/resources/resource_algebras.v
@@ -1,0 +1,25 @@
+From iris.algebra Require Import auth gmap dfrac.
+From iris.algebra.lib Require Import mono_list.
+From iris.bi.lib Require Import fractional.
+From aneris.lib Require Import gen_heap_light.
+From aneris.aneris_lang Require Import lang resources.
+From aneris.aneris_lang.lib Require Import lock_proof.
+From aneris.examples.snapshot_isolation.specs
+     Require Import user_params.
+From aneris.examples.snapshot_isolation.proof
+     Require Import time events.
+From aneris.examples.snapshot_isolation.proof
+     Require Import model.
+Import gen_heap_light.
+Import lock_proof.
+
+
+(* -------------------------------------------------------------------------- *)
+(** Some of Resource Algebras and global ghost names needed to define resources. *)
+
+(* TODO: add missing. *)
+Class IDBG Σ :=
+  { IDBG_Global_mem :>
+      inG Σ (authR (gen_heapUR Key (mono_listUR write_eventO)));
+    IDBG_lockG :> lockG Σ;
+  }.
