aneris/examples/snapshot_isolation/specs/resources.v
@@ -1,0 +1,107 @@
+From stdpp Require Import list.
+From iris.algebra Require Import frac.
+From iris.bi.lib Require Import fractional.
+From aneris.aneris_lang Require Export resources.
+From aneris.examples.reliable_communication.prelude
+     Require Import list_minus.
+From aneris.examples.snapshot_isolation.specs
+     Require Export user_params.
+
+Notation "h ≤ₛ h'" := (h `suffix_of` h') (at level 20).
+  
+Section Resources.
+
+  Definition Hist : Set := list val.
+
+  Reserved Notation "k ↦ₖ h" (at level 20).
+  Reserved Notation "k ↦{ c } vo" (at level 20).
+
+  Inductive local_state : Type :=
+   | CanStart
+   | Active (ms : gmap Key Hist).
+
+  Class SI_resources Mdl Σ
+    `{!anerisG Mdl Σ, !User_params}:= {
+
+    (** System global invariant *)
+    GlobalInv : iProp Σ;
+    GlobalInv_persistent :> Persistent GlobalInv;
+
+    (** Logical global points-to connective *)
+    OwnMemKey : Key → Hist → iProp Σ
+    where "k ↦ₖ h" := (OwnMemKey k h);
+    OwnMemKey_timeless k h :> Timeless (k ↦ₖ h);
+
+    (** Logical cache points-to connective *)
+    OwnLocalKey : Key → val → option val → iProp Σ
+    where "k ↦{ c } vo" := (OwnLocalKey k c vo);
+    OwnLocalKey_timeless k v c:> Timeless (k ↦{c} v);
+
+    (** Connection state *)
+    ConnectionState : val → local_state → iProp Σ;
+    
+    (** KVS resources *)
+    KVS_si : message → iProp Σ;
+    KVS_Init : iProp Σ;
+
+    (** Cache Key Status *)
+    KeyUpdStatus : val → Key → bool → iProp Σ;
+
+    (** Seen predciate *)
+    Seen : Key → Hist → iProp Σ;
+    Seen_timeless k h :> Timeless (Seen k h);
+    Seen_persistent k h :> Persistent (Seen k h);
+
+    (** Properties of points-to connective *)
+    OwnMemKey_exclusive k h h' :
+        k ↦ₖ h ⊢ k ↦ₖ h' -∗ False;
+
+    OwnLocalKey_exclusive k c v v' :
+        k ↦{c} v ⊢ k ↦{c} v' -∗ False;
+  
+    ConnectionState_relation E k r ms h :
+      ↑KVS_InvName ⊆ E ->
+      GlobalInv ⊢
+      ConnectionState r (Active ms) -∗ k ↦ₖ h ={E}=∗
+      ConnectionState r (Active ms) ∗ k ↦ₖ h ∗
+      ⌜k ∈ dom ms →
+      ∀ h', ms !! k = Some h' → h' ≤ₛ h ⌝;
+
+    OwnMemKey_OwnLocalKey_coh k h vo c E :
+        ↑KVS_InvName ⊆ E ->
+        h ≠ [] ->
+        GlobalInv ⊢
+        k ↦ₖ h -∗ k ↦{c} vo ={E}=∗ k ↦ₖ h -∗ k ↦{c} vo ∗ ⌜is_Some vo⌝;
+
+    ConnectionState_Keys E r ms :
+      ↑KVS_InvName ⊆ E ->
+        GlobalInv ⊢
+        ConnectionState r (Active ms) ={E}=∗
+        ConnectionState r (Active ms) ∗ ⌜dom ms ⊆ KVS_keys⌝;
+
+    OwnLocalKey_serializable E k cst v :
+      ↑KVS_InvName ⊆ E ->
+        GlobalInv ⊢
+        k ↦{cst} Some v ={E}=∗
+        k ↦{cst} Some v ∗ ⌜KVS_Serializable v⌝;
+
+    (** Properties of cache Key Status*)
+    KeyUpdStatus_exclusive c k b b' :
+      KeyUpdStatus c k b ⊢ KeyUpdStatus c k b' -∗ False;
+
+    (** Properties about the Seen predicate *) 
+    Seen_prefix k h h':
+      Seen k h ⊢ Seen k h' -∗ ⌜h ≤ₛ h' ∨ h' ≤ₛ h⌝;
+    
+    Seen_valid E k h h' : 
+       ↑KVS_InvName ⊆ E ->
+        GlobalInv ⊢
+        Seen k h ∗ k ↦ₖ h' ={E}=∗
+        k ↦ₖ h' ∗ ⌜h ≤ₛ h'⌝;
+  }.
+
+End Resources.
+(* Arguments SI_resources _ _ : clear implicits. *)
+
+Notation "k ↦ₖ h" := (OwnMemKey k h) (at level 20).
+Notation "k ↦{ c } vo" := (OwnLocalKey k c vo) (at level 20).
