aneris/examples/snapshot_isolation/specs/specs_deprecated/resources_hist.v
@@ -1,0 +1,115 @@
+From stdpp Require Import list.
+From iris.algebra Require Import frac.
+From iris.bi.lib Require Import fractional.
+From aneris.aneris_lang Require Export resources.
+From aneris.examples.reliable_communication.prelude
+     Require Import list_minus.
+From aneris.examples.snapshot_isolation.specs
+     Require Export user_params.
+
+Definition TObj : Set := (socket_address * gmap Key val).
+Definition THst : Set := list TObj.
+
+Definition at_origin (sa : socket_address) (h : THst) : THst :=
+  filter (λ x, fst x = sa) h.
+
+Definition can_commit (h : THst) (s : gmap Key val) (h' : THst) :=
+  ∀ (s' : TObj), s' ∈ list_minus h' h → dom s ## dom s'.2.
+
+Fixpoint get_val_at_key (h : THst) (k : Key) : option val :=
+ match h with
+ | [] => None
+ | t :: h' =>
+     match t.2 !! k with
+       | None => get_val_at_key h' k
+       | Some v => Some v
+     end
+ end.
+
+Definition get_current_state (h : THst) : gmap Key val :=
+  fold_right
+    (fun (mi : TObj) (m : gmap Key val) =>
+       merge (fun voi vo => if bool_decide (voi = None) then vo else voi)
+             mi.2 m) ∅ h.
+
+Lemma get_value_at_key_coh (h : THst) (k : Key) :
+  get_val_at_key h k = get_current_state h !! k.
+Proof. Admitted.
+
+Notation "h ≤ₚ h'" := (h `prefix_of` h') (at level 20).
+
+
+(** The idea of resources as predicates:
+
+GHist, Global Transaction History       :  [T0 T1 ... Ti ... T45 ... Tn]
+LHist, Local Client sa1 History         :  [   T1            T45]
+LHist, Local Client sa2 History         :  [T0        Ti]
+TState, Current Client sa1 T(n+1) state :  snapshot = Tn; cache={|k1 ↦ v1; ...|}
+
+*)
+
+Section Resources.
+
+  Class SI_resources Mdl Σ `{!anerisG Mdl Σ, !User_params}:= {
+
+    (** System global invariant *)
+    GlobalInv : iProp Σ;
+    GlobalInvPersistent :> Persistent GlobalInv;
+
+    (** Global history of committed transactions *)
+    GHist : THst → iProp Σ;
+
+    (** Local history of committed transactions *)
+    LHist : val → socket_address → THst → iProp Σ;
+
+    (** Local State of the current transaction containing the snapshot
+        and the effects of writes *)
+    TState : val → THst → gmap Key val → iProp Σ;
+
+    CanStart : socket_address → val → iProp Σ;
+
+    KVS_si : message → iProp Σ;
+
+    (** Laws *)
+    GHist_exclusive h h' :
+      GHist h ⊢ GHist h' -∗ False;
+
+    LHist_exclusive r sa h h' :
+      LHist r sa h ⊢ LHist r sa h' -∗ False;
+
+    LHist_origin r sa h :
+      LHist r sa h ⊢ ⌜∀ s, s ∈ h → s.1 = sa⌝;
+
+    TState_exclusive r h h' m m' :
+      TState r h m ⊢ TState r h' m' -∗ False;
+
+    GHist_LHist_relation E r sa h h' :
+    ↑KVS_InvName ⊆ E ->
+    GlobalInv ⊢ LHist r sa h -∗ GHist h' ={E}=∗
+    ⌜at_origin sa h' = h⌝;
+
+    GHist_Keys E h :
+    ↑KVS_InvName ⊆ E ->
+      GlobalInv ⊢ GHist h ={E}=∗
+      ⌜∀ s, s ∈ h → dom s.2 ⊆ KVS_keys⌝;
+
+    LHist_Keys E r sa h :
+    ↑KVS_InvName ⊆ E ->
+      GlobalInv ⊢ LHist r sa h ={E}=∗
+      ⌜∀ s, s ∈ h → dom s.2 ⊆ KVS_keys⌝;
+
+    TState_Keys E r h m :
+    ↑KVS_InvName ⊆ E ->
+      GlobalInv ⊢ TState r h m ={E}=∗ ⌜dom m ⊆ KVS_keys⌝;
+
+    (* This law is probably not needed. *)
+    (* GHist_LState_relation E cstate h h' s :
+    ↑KVS_InvName ⊆ E ->
+    GlobalInv ⊢ TState cstate h' s -∗ GHist h ={E}=∗
+    ⌜h ≤ₚ h'⌝; *)
+
+   }.
+
+End Resources.
+
+(* Arguments SI_resources _ _ : clear implicits. *)
