aneris/examples/snapshot_isolation/specs/specs_deprecated/resources_local_pointers.v
@@ -1,0 +1,82 @@
+From stdpp Require Import list.
+From iris.algebra Require Import frac.
+From iris.bi.lib Require Import fractional.
+From aneris.aneris_lang Require Export resources.
+From aneris.examples.reliable_communication.prelude
+     Require Import list_minus.
+From aneris.examples.snapshot_isolation.specs
+     Require Export user_params.
+From aneris.examples.snapshot_isolation.specs.specs_deprecated
+     Require Export events_local_pointers time.
+
+Section Resources.
+
+  Reserved Notation "k ↦ₖ e" (at level 20).
+  Reserved Notation "k ↦ₜ c" (at level 20).
+
+  Inductive local_state `{!KVS_time}: Type :=
+   | CanStart
+   | Active (ms : gmap Key (option write_event)).
+
+  Class SI_resources Mdl Σ
+    `{!anerisG Mdl Σ, !KVS_time, !User_params}:= {
+
+    (** System global invariant *)
+    GlobalInv : iProp Σ;
+    GlobalInvPersistent :> Persistent GlobalInv;
+
+    (** Logical global points-to connective *)
+    OwnMemKey : Key → option write_event → iProp Σ
+    where "k ↦ₖ v" := (OwnMemKey k v);
+
+   (** Logical Local points-to connective *)
+    OwnLocalKey : Key → cache_event → iProp Σ
+    where "k ↦ₜ c" := (OwnLocalKey k c);
+
+    (** Logical points-to connective *)
+    ConnectionState : val → local_state → iProp Σ;
+
+    KVS_si : message → iProp Σ;
+
+    (** Properties of points-to connective *)
+    OwnMemKey_timeless k v :> Timeless (k ↦ₖ v);
+    OwnMemKey_exclusive k v v' :
+      k ↦ₖ v ⊢ k ↦ₖ v' -∗ False;
+    OwnMemKey_key k we E :
+      nclose KVS_InvName ⊆ E →
+      GlobalInv ⊢
+      k ↦ₖ Some we ={E}=∗
+      k ↦ₖ Some we ∗ ⌜we_key we = k⌝;
+
+(** Properties of local points-to connective *)
+    OwnLocalKey_timeless k v :> Timeless (k ↦ₜ v);
+    OwnLocalKey_exclusive k v v' :
+      k ↦ₜ v ⊢ k ↦ₜ v' -∗ False;
+
+    (** Laws *)
+    ConnectionState_relation E k r ms we :
+    ↑KVS_InvName ⊆ E ->
+    GlobalInv ⊢
+    ConnectionState r (Active ms) -∗ k ↦ₖ Some we ={E}=∗
+    ⌜k ∈ dom ms →
+    ∀ we', ms !! k = Some (Some we') → we' ≤ₜ we ⌝;
+
+   OwnMemKey_OwnLocalKey_coh k we c E :
+      GlobalInv ⊢
+      k ↦ₖ Some we -∗ k ↦ₜ c ={E}=∗
+      ∃ we', ⌜c.(cache_snap) = Some we'⌝ ∗ ⌜we' ≤ₜ we⌝;
+
+   ConnectionState_Keys E r ms :
+    ↑KVS_InvName ⊆ E ->
+      GlobalInv ⊢
+      ConnectionState r (Active ms) ={E}=∗
+      ⌜dom ms ⊆ KVS_keys⌝;
+
+  (* ... about keys in domains *)
+  }.
+
+End Resources.
+(* Arguments SI_resources _ _ : clear implicits. *)
+
+Notation "k ↦ₖ e" := (OwnMemKey k e) (at level 20).
+Notation "k ↦ₜ c" := (OwnLocalKey k c) (at level 20).
