aneris/examples/snapshot_isolation/specs/specs_deprecated/resources_simpl.v
@@ -1,0 +1,53 @@
+From stdpp Require Import list.
+From iris.algebra Require Import frac.
+From iris.bi.lib Require Import fractional.
+From aneris.aneris_lang Require Export resources.
+From aneris.examples.reliable_communication.prelude
+     Require Import list_minus.
+From aneris.examples.snapshot_isolation.specs
+     Require Export user_params.
+
+Section Resources.
+
+  Reserved Notation "k ↦ₖ e" (at level 20).
+
+  Inductive local_state : Type :=
+   | CanStart
+   | Active (ms : gmap Key (option val)) (mc : gmap Key val).
+
+  Class SI_resources Mdl Σ
+        `{!anerisG Mdl Σ, !User_params}:= {
+
+    (** System global invariant *)
+    GlobalInv : iProp Σ;
+    GlobalInvPersistent :> Persistent GlobalInv;
+
+    (** Logical points-to connective *)
+    OwnMemKey : Key → option val → iProp Σ
+    where "k ↦ₖ v" := (OwnMemKey k v);
+
+    (** Logical points-to connective *)
+    ConnectionState : val → local_state → iProp Σ;
+
+    KVS_si : message → iProp Σ;
+
+    (** Properties of points-to connective *)
+    OwnMemKey_timeless k v :> Timeless (k ↦ₖ v);
+    OwnMemKey_exclusive k v v' :
+      k ↦ₖ v ⊢ k ↦ₖ v' -∗ False;
+
+    (** Laws *)
+
+    ConnectionState_Keys E r ms mc :
+    ↑KVS_InvName ⊆ E ->
+      GlobalInv ⊢
+      ConnectionState r (Active ms mc) ={E}=∗
+      ⌜dom ms ⊆ KVS_keys⌝ ∧ ⌜dom mc ⊆ dom ms⌝;
+
+  (* ... about keys in domains *)
+  }.
+
+End Resources.
+(* Arguments SI_resources _ _ : clear implicits. *)
+
+Notation "k ↦ₖ v" := (OwnMemKey k v) (at level 20).
