aneris/examples/snapshot_isolation/specs/specs_deprecated/specs_hist.v
@@ -1,0 +1,165 @@
+From iris.algebra Require Import auth gmap excl excl_auth.
+From aneris.algebra Require Import monotone.
+From aneris.aneris_lang Require Import network resources proofmode.
+From aneris.aneris_lang.lib Require Import
+     list_proof inject lock_proof.
+From aneris.aneris_lang.lib.serialization
+     Require Import serialization_proof.
+From aneris.aneris_lang.program_logic Require Import lightweight_atomic.
+From aneris.examples.snapshot_isolation
+     Require Import snapshot_isolation_code_api.
+From aneris.examples.snapshot_isolation.specs
+     Require Import user_params resources_hist.
+
+
+(** Specifications for read and write operations.  *)
+Section Specification.
+  Context `{!anerisG Mdl Σ, !User_params, !KVS_snapshot_isolation_api, !SI_resources Mdl Σ}.
+
+  Definition write_spec : Prop :=
+    ∀ (cstate : val) (sa : socket_address)
+      (h : THst) (m : gmap Key val) E
+      (k : Key) (v : SerializableVal),
+    ⌜k ∈ KVS_keys⌝ -∗
+    {{{ TState cstate h m }}}
+      SI_write cstate #k v @[ip_of_address sa] E
+    {{{ RET #(); TState cstate h (<[k:=v.(SV_val)]> m) }}}.
+
+  Definition read_spec : Prop :=
+    ∀ (cstate : val) (sa : socket_address)
+    (h : THst) (m : gmap Key val) E
+     (k : Key), ⌜k ∈ KVS_keys⌝ -∗
+    {{{ TState cstate h m }}}
+      SI_read cstate #k @[ip_of_address sa] E
+    {{{ (vo : val), RET vo; TState cstate h m ∗
+        ⌜k ∉ dom m ∧ vo = $(get_current_state h !! k) ∨
+         ∃ v, Some v = (m !! k) ∧ vo = $(Some v)⌝ }}}.
+
+  Definition start_spec : Prop :=
+    ∀ (cstate : val) (sa : socket_address) (E : coPset),
+    ⌜↑KVS_InvName ⊆ E⌝ -∗
+    <<< ∀∀ (hl hg: THst),
+        LHist cstate sa hl ∗ GHist hg ∗ CanStart sa cstate >>>
+      SI_start cstate @[ip_of_address sa] E
+    <<<▷ RET #();
+        LHist cstate sa hl ∗ GHist hg ∗ TState cstate hg ∅ >>>.
+
+  Definition commit_spec : Prop :=
+   ∀ (cstate : val) (sa : socket_address)
+     (P : THst → iProp Σ)
+     (Q : THst → gmap Key val → iProp Σ)
+    (E : coPset),
+    ⌜↑KVS_InvName ⊆ E⌝ -∗
+    <<< ∀∀ (hl hs hg: THst) (m : gmap Key val),
+    LHist cstate sa hl ∗ GHist hg ∗ TState cstate hs m ∗ P hs >>>
+      SI_commit cstate @[ip_of_address sa] E
+    <<<▷∃∃ b, RET #b;
+          CanStart sa cstate ∗
+          (⌜b = true⌝ ∗ ⌜can_commit hs m hg⌝ ∗
+            GHist ((sa, m) :: hg) ∗ LHist cstate sa ((sa, m) :: hl) ∗ Q hs m) ∨
+          (⌜b = false⌝ ∗ ⌜¬ can_commit hs m hg⌝ ∗
+            GHist hg ∗ LHist cstate sa hl) >>>.
+
+(** TODO: Read only transaction *)
+
+Definition run_spec : Prop :=
+    ∀ (cstate : val) (tbody : val)
+      (sa : socket_address) (E : coPset)
+      (m : gmap Key val) (h: THst) (hl : THst)
+      (P : THst → iProp Σ)
+      (Q : THst → gmap Key val → iProp Σ),
+    ⌜↑KVS_InvName ⊆ E⌝
+    -∗
+    {{{ TState cstate h ∅ ∗ P h }}}
+      tbody cstate #() @[ip_of_address sa] E
+    {{{ RET #(); TState cstate h m ∗ Q h m }}}
+    →
+    <<< ∀∀ (x : unit), CanStart sa cstate ∗ GHist h ∗ LHist cstate sa hl ∗ P h >>>
+           SI_run cstate tbody @[ip_of_address sa] E
+    <<<▷∃∃ b h',  RET #b;
+        ⌜h ≤ₚ h'⌝ ∗
+        CanStart sa cstate ∗
+        (⌜b = true⌝ ∗ ⌜can_commit h m h'⌝ ∗
+                      GHist ((sa, m) :: h') ∗ LHist cstate sa ((sa, m) :: hl) ∗ Q h m) ∨
+        (⌜b = false⌝ ∗ ⌜¬ can_commit h m h'⌝ ∗ GHist h' ∗ LHist cstate sa hl) >>>.
+
+  Definition init_client_proxy_spec : Prop :=
+    ∀ (sa : socket_address),
+    {{{ unallocated {[sa]} ∗
+        KVS_address ⤇ KVS_si ∗
+        sa ⤳ (∅, ∅) ∗
+        free_ports (ip_of_address sa) {[port_of_address sa]} }}}
+      SI_init_client_proxy (s_serializer KVS_serialization)
+                  #sa #KVS_address @[ip_of_address sa]
+    {{{ cstate, RET cstate; CanStart sa cstate }}}.
+
+Definition init_kvs_spec : Prop :=
+  {{{ KVS_address ⤇ KVS_si ∗
+        KVS_address ⤳ (∅,∅) ∗
+        free_ports (ip_of_address KVS_address)
+                   {[port_of_address KVS_address]} }}}
+      SI_init_server (s_serializer KVS_serialization)
+        #KVS_address
+        @[(ip_of_address KVS_address)]
+    {{{ RET #(); True }}}.
+
+End Specification.
+
+
+Class KVSG  Σ :=
+  {
+    KVS_lockG :> lockG Σ;
+    (* TODO ... : ... ; *)
+  }.
+
+Definition KVSΣ : gFunctors :=
+  #[ (* TODO ... ; *) lockΣ].
+
+Instance subG_DBΣ {Σ} : subG KVSΣ Σ → KVSG Σ.
+Proof. econstructor; solve_inG. Qed.
+
+Section SI_Module.
+  Context `{!anerisG Mdl Σ}.
+
+  Class SI_init `{!User_params, !KVS_snapshot_isolation_api} := {
+     SI_init_module E :
+        True ⊢ |={E}=> ∃ (SIRes : SI_resources Mdl Σ),
+       GlobalInv ∗
+       GHist [] ∗
+       ⌜init_kvs_spec⌝ ∗
+       ⌜init_client_proxy_spec⌝ ∗
+       ⌜read_spec⌝ ∗
+       ⌜write_spec⌝ ∗
+       ⌜start_spec⌝ ∗
+       ⌜commit_spec⌝ ∗
+       ⌜run_spec⌝ }.
+
+End SI_Module.
+
+(* TODO: REMOVE THIS LATER, it's just an example of usage. *)
+Section Prove_of_t_body_of_some_example.
+  Context `{!anerisG Mdl Σ}.
+  Context `{!User_params, !KVS_snapshot_isolation_api, !SI_resources Mdl Σ}.
+  Context (rd_spec : read_spec).
+
+  Definition code_snippet : val :=
+    λ: "cstate" "k", SI_read "cstate" "k".
+
+  Lemma code_snippet_proof sa (cstate : val) h m (k : Key) :
+     {{{ ⌜k ∈ KVS_keys⌝ ∗
+           TState cstate h (<[k:=#42]> m)}}}
+       code_snippet cstate #k @[ip_of_address sa]
+     {{{ vo, RET vo; ⌜vo = $(Some 42)⌝ }}}.
+ Proof.
+   rewrite /code_snippet.
+   iIntros (Φ) "(Hkey & HTState) HΦ".
+   wp_pures.
+   iApply (rd_spec with "[$][$HTState]").
+   iNext.
+   iIntros (vo) "(_ & [%Habs | %Hpost])"; iApply "HΦ";
+     first by set_solver.
+   destruct Hpost as (v & Hv & Hvo).
+   by simplify_map_eq /=.
+ Qed.
+
+End Prove_of_t_body_of_some_example.
