aneris/examples/snapshot_isolation/specs/specs_deprecated/specs_points_to_with_key_status.v
@@ -1,0 +1,198 @@
+From iris.algebra Require Import auth gmap excl excl_auth.
+From aneris.algebra Require Import monotone.
+From aneris.aneris_lang Require Import network resources proofmode.
+From aneris.aneris_lang.lib Require Import
+     list_proof inject lock_proof.
+From aneris.aneris_lang.lib.serialization
+     Require Import serialization_proof.
+From aneris.aneris_lang.program_logic Require Import lightweight_atomic.
+From aneris.examples.snapshot_isolation
+     Require Import snapshot_isolation_code_api.
+From aneris.examples.snapshot_isolation.specs
+     Require Import user_params resources_points_to_with_key_status.
+From aneris.examples.snapshot_isolation.specs.specs_deprecated
+     Require Import time events.
+
+Definition can_commit_set `{!KVS_time}
+ (m ms : gmap Key (option write_event)) (s : gset Key) : Prop :=
+  ∀ (k : Key), k ∈ s → m !! k = ms !! k.
+
+Definition can_commit `{!KVS_time}
+ (m ms : gmap Key (option write_event)) (mc : gmap Key (option val * bool)) : Prop :=
+  ∀ (k : Key) (v: val), mc !! k = Some (Some v, true) → m !! k = ms !! k.
+
+Definition max_timestamp `{!KVS_time} t (m : gmap Key (option write_event)) : Prop :=
+    ∀ k (e : write_event), m !! k = Some (Some e) → TM_lt e.(we_time) t.
+
+Definition weo_val `{!KVS_time} (weo : option write_event) :=
+    match weo with
+      | None => None
+      | Some we => Some we.(we_val)
+    end.
+
+Definition commit_event `{!KVS_time}
+  (k : Key) (t : Time) (p : option val * bool) (eo : option write_event) :=
+    match p with
+    | (Some v, true) => Some {|we_key:=k; we_val:=v; we_time:=t|}
+    | _              => eo
+    end.
+
+(** Specifications for read and write operations.  *)
+Section Specification.
+  Context `{!anerisG Mdl Σ, !User_params, !KVS_time,
+            !KVS_snapshot_isolation_api, !SI_resources Mdl Σ}.
+
+  Definition write_spec : iProp Σ :=
+    ∀ (c : val) (sa : socket_address)
+      (vo : option val)
+      (k : Key) (v : SerializableVal) (b : bool) E,
+    ⌜k ∈ KVS_keys⌝ -∗
+    {{{ k ↦{c} vo ∗ KeyUpdStatus c k b}}}
+      SI_write c #k v @[ip_of_address sa] E
+    {{{ RET #(); k ↦{c} Some v.(SV_val) ∗ KeyUpdStatus c k true }}}.
+
+  Definition read_spec : iProp Σ :=
+    ∀ (c : val) (sa : socket_address)
+      (k : Key) (vo : option val) E,
+    ⌜k ∈ KVS_keys⌝ -∗
+    {{{ k ↦{c} vo }}}
+      SI_read c #k @[ip_of_address sa] E
+    {{{ RET $vo; k ↦{c} vo }}}.
+
+   Definition start_spec : iProp Σ :=
+    ∀ (c : val) (sa : socket_address)
+       (E : coPset),
+    ⌜↑KVS_InvName ⊆ E⌝ -∗
+    <<< ∀∀ (m : gmap Key (option write_event)),
+       ConnectionState c CanStart ∗
+       [∗ map] k ↦ eo ∈ m, k ↦ₖ eo >>>
+      SI_start c @[ip_of_address sa] E
+    <<<▷ RET #();
+       ConnectionState c (Active m) ∗
+       ([∗ map] k ↦ eo ∈ m, k ↦ₖ eo) ∗
+       ([∗ map] k ↦ eo ∈ m, k ↦{c} (weo_val eo) ∗ KeyUpdStatus c k false)>>>.
+
+  Definition commit_spec : iProp Σ :=
+   ∀ (c : val) (sa : socket_address)
+     (E : coPset),
+    ⌜↑KVS_InvName ⊆ E⌝ -∗
+    <<< ∀∀ (m ms: gmap Key (option write_event))
+           (mc : gmap Key (option val * bool)),
+        ConnectionState c (Active ms) ∗
+        ⌜dom m = dom ms⌝ ∗ ⌜dom ms = dom mc⌝ ∗
+        ([∗ map] k ↦ eo ∈ m, k ↦ₖ eo) ∗
+        ([∗ map] k ↦ p ∈ mc, k ↦{c} p.1  ∗ KeyUpdStatus c k p.2) >>>
+      SI_commit c @[ip_of_address sa] E
+    <<<▷∃∃ b, RET #b;
+        ConnectionState c CanStart ∗
+        (** Transaction has been commited. *)
+        ((⌜b = true⌝ ∗ ⌜can_commit m ms mc⌝ ∗
+         ∃ (t: Time), ⌜max_timestamp t m⌝ ∗
+          ([∗ map] k↦ eo;p ∈ m; mc, k ↦ₖ commit_event k t p eo)) ∨
+        (** Transaction has been aborted. *)
+         (⌜b = false⌝ ∗ ⌜¬ can_commit m ms mc⌝ ∗
+           [∗ map] k ↦ eo ∈ m, k ↦ₖ eo)) >>>.
+
+Definition run_spec : iProp Σ :=
+    ∀ (c : val) (tbody : val)
+      (sa : socket_address) (E : coPset)
+      (P :  gmap Key (option write_event) → iProp Σ)
+      (Q :  gmap Key (option write_event) → gmap Key (option val * bool) → iProp Σ),
+    ⌜↑KVS_InvName ⊆ E⌝ -∗
+      (∀ (m0 : gmap Key (option write_event)) (mc : gmap Key (option val * bool)),
+         {{{ ([∗ map] k ↦ eo ∈ m0, k ↦{c} (weo_val eo) ∗ KeyUpdStatus c k false) ∗ P m0 }}}
+           tbody c #() @[ip_of_address sa] E
+         {{{ RET #(); ([∗ map] k ↦ p ∈ mc, k ↦{c} p.1 ∗ KeyUpdStatus c k p.2) ∗ Q m0 mc }}})
+    →
+    <<< ∀∀ m0, ConnectionState c CanStart ∗
+               P m0 ∗
+               [∗ map] k ↦ eo ∈ m0, k ↦ₖ eo >>>
+           SI_run c tbody @[ip_of_address sa] E
+    <<<▷∃∃ m1 mc b, RET #b;
+               ConnectionState c CanStart ∗
+               (** Transaction has been commited. *)
+               ((⌜b = true⌝ ∗ ⌜can_commit m1 m0 mc⌝ ∗ Q m0 mc ∗
+                ∃ (t: Time), ⌜max_timestamp t m1⌝ ∗
+                   ([∗ map] k↦ eo;p ∈ m1; mc, k ↦ₖ commit_event k t p eo)) ∨
+               (** Transaction has been aborted. *)
+               (⌜b = false⌝ ∗ ⌜¬ can_commit m1 m0 mc⌝ ∗
+                [∗ map] k ↦ eo ∈ m1, k ↦ₖ eo)) >>>.
+
+ Definition commit_spec_alt : iProp Σ :=
+   ∀ (c : val) (sa : socket_address)
+     (E : coPset),
+    ⌜↑KVS_InvName ⊆ E⌝ -∗
+    <<< ∀∀ (m ms: gmap Key (option write_event))
+           (mcr : gmap Key (option val))
+           (mcw : gmap Key val),
+        ConnectionState c (Active ms) ∗
+        ⌜dom m = dom ms⌝ ∗ ⌜dom ms = dom mcr ∪ dom mcw⌝ ∗ ⌜dom mcr ## dom mcw⌝ ∗
+        ([∗ map] k ↦ eo ∈ m, k ↦ₖ eo) ∗
+        ([∗ map] k ↦ vo ∈ mcr, k ↦{c}  vo    ∗ KeyUpdStatus c k false) ∗
+        ([∗ map] k ↦ v  ∈ mcw, k ↦{c} Some v ∗ KeyUpdStatus c k true) >>>
+      SI_commit c @[ip_of_address sa] E
+    <<<▷∃∃ b, RET #b;
+        ConnectionState c CanStart ∗
+        (** Transaction has been commited. *)
+        ((⌜b = true⌝ ∗ ⌜can_commit_set m ms (dom mcw)⌝ ∗
+         ∃ (t: Time), ⌜max_timestamp t m⌝ ∗
+          ([∗ map] k↦_ ∈ mcr, ∃ eo, ⌜m !! k = Some eo⌝ ∗ k ↦ₖ eo) ∗
+          ([∗ map] k↦v ∈ mcw, k ↦ₖ Some {|we_key:=k; we_val:=v; we_time:=t|})) ∨
+        (** Transaction has been aborted. *)
+         (⌜b = false⌝ ∗ ⌜¬ can_commit_set m ms (dom mcw)⌝ ∗
+           [∗ map] k ↦ eo ∈ m, k ↦ₖ eo)) >>>.
+
+  Definition init_client_proxy_spec : iProp Σ :=
+    ∀ (sa : socket_address),
+    {{{ unallocated {[sa]} ∗
+        KVS_address ⤇ KVS_si ∗
+        sa ⤳ (∅, ∅) ∗
+        free_ports (ip_of_address sa) {[port_of_address sa]} }}}
+      SI_init_client_proxy (s_serializer KVS_serialization)
+                  #sa #KVS_address @[ip_of_address sa]
+    {{{ cstate, RET cstate; ConnectionState cstate CanStart }}}.
+
+Definition init_kvs_spec : iProp Σ :=
+  {{{ KVS_address ⤇ KVS_si ∗
+        KVS_address ⤳ (∅,∅) ∗
+        free_ports (ip_of_address KVS_address)
+                   {[port_of_address KVS_address]} ∗
+      KVS_Init }}}
+      SI_init_server (s_serializer KVS_serialization)
+        #KVS_address
+        @[(ip_of_address KVS_address)]
+    {{{ RET #(); True }}}.
+
+End Specification.
+
+
+Class KVSG  Σ :=
+  {
+    KVS_lockG :> lockG Σ;
+    (* TODO ... : ... ; *)
+  }.
+
+Definition KVSΣ : gFunctors :=
+  #[ (* TODO ... ; *) lockΣ].
+
+Instance subG_KVSΣ {Σ} : subG KVSΣ Σ → KVSG Σ.
+Proof. econstructor; solve_inG. Qed.
+
+Section SI_Module.
+  Context `{!anerisG Mdl Σ, !KVS_time}.
+
+  Class SI_init `{!User_params, !KVS_snapshot_isolation_api} := {
+     SI_init_module E :
+        True ⊢ |={E}=> ∃ (SIRes : SI_resources Mdl Σ),
+       GlobalInv ∗
+       ([∗ set] k ∈ KVS_keys, k ↦ₖ None) ∗
+       init_kvs_spec ∗
+       KVS_Init ∗
+       init_client_proxy_spec ∗
+       read_spec ∗
+       write_spec ∗
+       start_spec ∗
+       commit_spec ∗
+       run_spec }.
+
+End SI_Module.
