aneris/examples/snapshot_isolation/specs/specs_deprecated/specs_without_local_points_to.v
@@ -1,0 +1,216 @@
+From iris.algebra Require Import auth gmap excl excl_auth.
+From aneris.algebra Require Import monotone.
+From aneris.aneris_lang Require Import network resources proofmode.
+From aneris.aneris_lang.lib Require Import
+     list_proof inject lock_proof.
+From aneris.aneris_lang.lib.serialization
+     Require Import serialization_proof.
+From aneris.aneris_lang.program_logic Require Import lightweight_atomic.
+From aneris.examples.snapshot_isolation
+     Require Import snapshot_isolation_code_api.
+From aneris.examples.snapshot_isolation.specs
+     Require Import user_params.
+From aneris.examples.snapshot_isolation.specs.specs_deprecated
+     Require Import time events resources_without_local_points_to.
+
+
+(** Specifications for read and write operations.  *)
+Section Specification.
+  Context `{!anerisG Mdl Σ, !User_params, !KVS_time,
+            !KVS_snapshot_isolation_api, !SI_resources Mdl Σ}.
+
+  Definition write_spec : Prop :=
+    ∀ (cstate : val) (sa : socket_address)
+      (ms : gmap Key (option write_event))
+      (mc : gmap Key val) E
+      (k : Key) (v : SerializableVal),
+    ⌜k ∈ KVS_keys⌝ -∗
+    {{{ ConnectionState cstate (Active ms mc) }}}
+      SI_write cstate #k v @[ip_of_address sa] E
+    {{{ RET #();
+        ConnectionState cstate (Active ms (<[k:= v.(SV_val)]> mc)) }}}.
+
+  Definition read_spec : Prop :=
+    ∀ (cstate : val) (sa : socket_address)
+      (ms : gmap Key (option write_event))
+      (mc : gmap Key val)
+      (eo : option write_event) E
+     (k : Key), ⌜ms !! k = Some eo⌝ -∗
+    {{{ ConnectionState cstate (Active ms mc) }}}
+      SI_read cstate #k @[ip_of_address sa] E
+    {{{ (ro : val), RET $ro; ConnectionState cstate (Active ms mc) ∗
+        ⌜(k ∉ dom mc ∧
+        match eo with
+           | (Some we) => ro = SOMEV we.(we_val)
+           | None => ro = NONEV
+         end) ∨
+        ∃ v, Some v = (mc !! k) ∧ ro = $(Some v)⌝ }}}.
+
+  Definition start_spec : Prop :=
+    ∀ (cstate : val) (sa : socket_address)
+       (E : coPset),
+    ⌜↑KVS_InvName ⊆ E⌝ -∗
+    <<< ∀∀ (m : gmap Key (option write_event)),
+       ConnectionState cstate CanStart ∗
+       [∗ map] k ↦ eo ∈ m, k ↦ₖ eo >>>
+      SI_start cstate @[ip_of_address sa] E
+    <<<▷ RET #();
+       ConnectionState cstate (Active m ∅) ∗
+       [∗ map] k ↦ eo ∈ m, k ↦ₖ eo >>>.
+
+  Definition can_commit
+    (m ms : gmap Key (option write_event))
+    (mc : gmap Key val) : Prop :=
+    ∀ k, is_Some (mc !! k) → ms !! k = m !! k.
+
+  Definition max_timestamp t (m : gmap Key (option write_event)) : Prop :=
+    ∀ k (e : write_event), m !! k = Some (Some e) → TM_lt e.(we_time) t.
+
+  Definition commit_spec : Prop :=
+   ∀ (cstate : val) (sa : socket_address)
+     (P :  gmap Key (option write_event) → iProp Σ)
+     (Q :  gmap Key (option write_event) → gmap Key val → iProp Σ)
+     (E : coPset),
+    ⌜↑KVS_InvName ⊆ E⌝ -∗
+    <<< ∀∀ (m ms: gmap Key (option write_event)) (mc : gmap Key val),
+        ConnectionState cstate (Active ms mc) ∗
+        [∗ map] k ↦ eo ∈ m, k ↦ₖ eo ∗ P ms >>>
+      SI_commit cstate @[ip_of_address sa] E
+    <<<▷∃∃ b, RET #b;
+        ConnectionState cstate CanStart ∗
+        (** Transaction has been commited. *)
+        (⌜b = true⌝ ∗ ⌜can_commit m ms mc⌝ ∗
+          ∃ (t: Time),
+            (** Pointers that have been only read *)
+           ([∗ set] k ∈ (dom m) ∖ (dom mc),
+              let write_evento :=
+              match (m !! k) with
+                | None => None
+                | Some write_evento => write_evento
+              end in k ↦ₖ write_evento) ∗
+            (** Pointers that have been written to *)
+            ([∗ map] k↦v ∈ mc,
+               k ↦ₖ Some {| we_key := k; we_val := v; we_time := t |}) ∗
+             ⌜max_timestamp t m⌝ ∗ Q ms mc) ∨
+        (** Transaction has been aborted. *)
+         (⌜b = false⌝ ∗ ⌜¬ can_commit m ms mc⌝ ∗
+           [∗ map] k ↦ eo ∈ m, k ↦ₖ eo) >>>.
+
+Definition run_spec : Prop :=
+    ∀ (cstate : val) (tbody : val)
+      (sa : socket_address) (E : coPset)
+      (P :  gmap Key (option write_event) → iProp Σ)
+      (Q :  gmap Key (option write_event) → gmap Key val → iProp Σ),
+    ⌜↑KVS_InvName ⊆ E⌝
+    -∗
+      (∀ ms mc,
+    {{{ ConnectionState cstate (Active ms ∅) ∗ P ms }}}
+      tbody cstate #() @[ip_of_address sa] E
+    {{{ RET #(); ConnectionState cstate (Active ms mc) ∗ Q ms mc }}})
+    →
+    <<< ∀∀ m0,
+        ConnectionState cstate CanStart ∗ P m0 ∗
+          [∗ map] k ↦ eo ∈ m0, k ↦ₖ eo >>>
+           SI_run cstate tbody @[ip_of_address sa] E
+    <<<▷∃∃ m1 mc b,  RET #b;
+        (** TODO : coh(m0,m1) = m0 *)
+        ConnectionState cstate CanStart ∗
+        (** Transaction has been commited. *)
+        (⌜b = true⌝ ∗ ⌜can_commit m1 m0 mc⌝ ∗
+          ∃ (t: Time),
+            (** Pointers that have been only read *)
+           ([∗ set] k ∈ (dom m1) ∖ (dom mc),
+              let write_evento :=
+              match (m0 !! k) with
+                | None => None
+                | Some write_evento => write_evento
+              end in k ↦ₖ write_evento) ∗
+            (** Pointers that have been written to *)
+            ([∗ map] k↦v ∈ mc,
+               k ↦ₖ Some {| we_key := k; we_val := v; we_time := t |}) ∗
+             ⌜max_timestamp t m1⌝ ∗ Q m0 mc) ∨
+        (** Transaction has been aborted. *)
+         (⌜b = false⌝ ∗ ⌜¬ can_commit m1 m0 mc⌝ ∗
+           [∗ map] k ↦ eo ∈ m1, k ↦ₖ eo) >>>.
+
+  Definition init_client_proxy_spec : Prop :=
+    ∀ (sa : socket_address),
+    {{{ unallocated {[sa]} ∗
+        KVS_address ⤇ KVS_si ∗
+        sa ⤳ (∅, ∅) ∗
+        free_ports (ip_of_address sa) {[port_of_address sa]} }}}
+      SI_init_client_proxy (s_serializer KVS_serialization)
+                  #sa #KVS_address @[ip_of_address sa]
+    {{{ cstate, RET cstate; ConnectionState cstate CanStart }}}.
+
+Definition init_kvs_spec : Prop :=
+  {{{ KVS_address ⤇ KVS_si ∗
+        KVS_address ⤳ (∅,∅) ∗
+        free_ports (ip_of_address KVS_address)
+                   {[port_of_address KVS_address]} }}}
+      SI_init_server (s_serializer KVS_serialization)
+        #KVS_address
+        @[(ip_of_address KVS_address)]
+    {{{ RET #(); True }}}.
+
+End Specification.
+
+
+Class KVSG  Σ :=
+  {
+    KVS_lockG :> lockG Σ;
+    (* TODO ... : ... ; *)
+  }.
+
+Definition KVSΣ : gFunctors :=
+  #[ (* TODO ... ; *) lockΣ].
+
+Instance subG_DBΣ {Σ} : subG KVSΣ Σ → KVSG Σ.
+Proof. econstructor; solve_inG. Qed.
+
+Section SI_Module.
+  Context `{!anerisG Mdl Σ, !KVS_time}.
+
+  Class SI_init `{!User_params, !KVS_snapshot_isolation_api} := {
+     SI_init_module E :
+        True ⊢ |={E}=> ∃ (SIRes : SI_resources Mdl Σ),
+       GlobalInv ∗
+       ([∗ set] k ∈ KVS_keys, k ↦ₖ None) ∗
+       ⌜init_kvs_spec⌝ ∗
+       ⌜init_client_proxy_spec⌝ ∗
+       ⌜read_spec⌝ ∗
+       ⌜write_spec⌝ ∗
+       ⌜start_spec⌝ ∗
+       ⌜commit_spec⌝ ∗
+       ⌜run_spec⌝ }.
+
+End SI_Module.
+
+(* TODO: REMOVE THIS LATER, it's just an example of usage. *)
+Section Prove_of_t_body_of_some_example.
+  Context `{!anerisG Mdl Σ}.
+  Context `{!User_params, !KVS_time, !KVS_snapshot_isolation_api, !SI_resources Mdl Σ}.
+  Context (rd_spec : read_spec).
+
+  Definition code_snippet : val :=
+    λ: "cstate" "k", SI_read "cstate" "k".
+
+  Lemma code_snippet_proof sa (cstate : val) ms m (k : Key) :
+     {{{ ⌜k ∈ dom ms⌝ ∗
+           ConnectionState cstate (Active ms (<[k:=#42]> m))}}}
+       code_snippet cstate #k @[ip_of_address sa]
+     {{{ vo, RET vo; ⌜vo = $(Some 42)⌝ }}}.
+ Proof.
+   rewrite /code_snippet.
+   iIntros (Φ) "(%Hkey & HConnectionState) HΦ".
+   wp_pures.
+   iApply (rd_spec with "[][$HConnectionState]").
+   - iPureIntro. admit.
+   - iNext.
+   iIntros (vo) "(_ & [%Habs | %Hpost])"; iApply "HΦ".
+   -- admit.
+   -- destruct Hpost as (v & Hv & Hvo).
+      by simplify_map_eq /=.
+ Admitted.
+
+End Prove_of_t_body_of_some_example.
