aneris/examples/snapshot_isolation/util/util_proof.v
@@ -1,0 +1,323 @@
+From aneris.examples.snapshot_isolation.util Require Import util_code.
+From aneris.aneris_lang Require Import tactics adequacy proofmode.
+From aneris.examples.snapshot_isolation.specs
+     Require Import user_params resources specs.
+From aneris.examples.snapshot_isolation.instantiation
+      Require Import snapshot_isolation_api_implementation.
+From aneris.aneris_lang.program_logic Require Import lightweight_atomic.
+From iris.algebra Require Import gmap.
+From iris.algebra Require Import excl.
+
+
+Section proof.
+
+Context `{!anerisG Mdl Σ, !User_params, !KVSG Σ, !SI_resources Mdl Σ,
+           !SI_client_toolbox}.
+
+  Lemma commitU_spec :
+    ∀ c sa E,
+    ⌜↑KVS_InvName ⊆ E⌝ -∗
+    <<< ∀∀ (m ms: gmap Key Hist)
+           (mc : gmap Key (option val * bool)),
+        ConnectionState c (Active ms) ∗
+        ⌜dom m = dom ms⌝ ∗ ⌜dom ms = dom mc⌝ ∗
+        ([∗ map] k ↦ h ∈ m, k ↦ₖ h) ∗
+        ([∗ map] k ↦ p ∈ mc, k ↦{c} p.1  ∗ KeyUpdStatus c k p.2) >>>
+      commitU c @[ip_of_address sa] E
+    <<<▷ RET #();
+        ConnectionState c CanStart ∗
+        (** Transaction has been commited. *)
+        ((⌜can_commit m ms mc⌝ ∗
+          ([∗ map] k↦ h;p ∈ m; mc, 
+            k ↦ₖ commit_event p h ∗ Seen k (commit_event p h))) ∨
+        (** Transaction has been aborted. *)
+         (⌜¬ can_commit m ms mc⌝ ∗
+           [∗ map] k ↦ h ∈ m, k ↦ₖ h ∗ Seen k h)) >>>.
+  Proof.
+    iIntros (cst sa E name Φ) "!>HΦ".
+    rewrite/commitU.
+    wp_pures.
+    wp_apply (SI_commit_spec with "[//] [HΦ]").
+    iMod "HΦ" as "(%m & %ms & %mc & pre & HΦ)".
+    iModIntro.
+    iExists m, ms, mc.
+    iSplitL "pre"; first done.
+    iIntros "!>%b (CanStart & [( _ & post)|(_ & post)])"; 
+    iMod ("HΦ" with "[$CanStart $post]") as "HΦ";
+    iModIntro;
+    by wp_pures.
+  Qed.
+
+  Lemma commitT_spec :
+    ∀ c sa E,
+    ⌜↑KVS_InvName ⊆ E⌝ -∗
+    <<< ∀∀ (m ms: gmap Key Hist)
+           (mc : gmap Key (option val * bool)),
+        ⌜can_commit m ms mc⌝ ∗
+        ConnectionState c (Active ms) ∗
+        ⌜dom m = dom ms⌝ ∗ ⌜dom ms = dom mc⌝ ∗
+        ([∗ map] k ↦ h ∈ m, k ↦ₖ h) ∗
+        ([∗ map] k ↦ p ∈ mc, k ↦{c} p.1  ∗ KeyUpdStatus c k p.2) >>>
+      commitT c @[ip_of_address sa] E
+    <<<▷ RET #();
+        ConnectionState c CanStart ∗
+        (** Transaction has been commited. *)
+        ([∗ map] k↦ h;p ∈ m; mc, 
+            k ↦ₖ commit_event p h ∗ Seen k (commit_event p h)) >>>.
+  Proof.
+    iIntros (cst sa E name Φ) "!>HΦ".
+    rewrite/commitT/assert.
+    wp_pures.
+    wp_apply (SI_commit_spec with "[//] [HΦ]").
+    iMod "HΦ" as "(%m & %ms & %mc & (%can_commit & pre) & HΦ)".
+    iModIntro.
+    iExists m, ms, mc.
+    iSplitL "pre"; first done.
+    iIntros "!>%b (CanStart & [(-> & _ & post)|(_ & %abs & _)])"; try done.
+    iMod ("HΦ" with "[$CanStart $post]") as "HΦ".
+    iModIntro.
+    by wp_pures.
+  Qed.
+
+  Lemma wait_on_keyT_spec :
+    ∀ (c cond : val) (k : Key) ms sa E (P P_tok : iProp Σ)
+      (Q : val → iProp Σ) (Q_tok φ : _ → _ → _ → iProp Σ),
+    ⌜↑KVS_InvName ⊆ E⌝ -∗
+    ⌜dom ms ⊆ KVS_keys⌝ -∗
+    ⌜k ∈ dom ms⌝ -∗
+    □ (∀ v h, P_tok ∗ Q v ∗ Seen k (v :: h) ={⊤, E}=∗
+          ∃ m, ⌜dom m = dom ms⌝ ∗ ([∗ map] k ↦ h ∈ m, k ↦ₖ h) ∗ φ m v h ∗ Q_tok m v h ∗
+            ▷ (([∗ map] k ↦ h ∈ m, k ↦ₖ h) ∗ Q_tok m v h ={E, ⊤}=∗ emp)) -∗
+    □ (|={⊤, E}=> ∃ m, ⌜dom m = dom ms⌝ ∗
+          ([∗ map] k ↦ h ∈ m, k ↦ₖ h) ∗
+            ▷ (([∗ map] k ↦ h ∈ m, k ↦ₖ h) ={E, ⊤}=∗ emp)) -∗
+    (∀ m v', {{{ P ∗ ConnectionState c (Active m) ∗ ⌜dom m = dom ms⌝ ∗
+              ([∗ map] k ↦ h ∈ m, k ↦{c} (hist_val h) ∗ KeyUpdStatus c k false)
+            }}}
+            cond v' @[ip_of_address sa]
+            {{{ m' (b : bool), RET #b;
+              ConnectionState c (Active m') ∗ ⌜dom m' = dom ms⌝ ∗
+              ([∗ map] k ↦ h ∈ m', k ↦{c} (hist_val h) ∗ KeyUpdStatus c k false) ∗
+              if b then Q v' else P
+            }}}) -∗
+    {{{
+      P ∗ P_tok ∗ ConnectionState c (Active ms) ∗
+      ([∗ map] k ↦ h ∈ ms, k ↦{c} (hist_val h) ∗ KeyUpdStatus c k false) ∗
+      ([∗ map] k ↦ h ∈ ms, Seen k h)
+    }}}
+     wait_on_keyT c cond #k @[ip_of_address sa]
+    {{{ m v h, RET #(); ⌜dom m = dom ms⌝ ∗ φ m v h ∗
+      ConnectionState c (Active m) ∗
+      ([∗ map] k ↦ h ∈ m, k ↦{c} (hist_val h) ∗ KeyUpdStatus c k false) ∗
+      ([∗ map] k ↦ h ∈ m, Seen k h)
+    }}}.
+  Proof.
+    iIntros (c cond k ms sa E P P_tok Q Q_tok) "%φ %name %ms_keys %k_ms #finish
+      #inv #cond_spec %Φ !> (P & P_tok & Active & cache & Seen) HΦ".
+    rewrite/wait_on_keyT.
+    wp_pures.
+    iRevert (ms ms_keys k_ms) "inv finish cond_spec HΦ cache Active P Seen".
+    iLöb as "IH".
+    iIntros (ms ms_keys k_ms) "#inv #finish #cond_spec HΦ cache Active P #Seen".
+    move: ((proj1 (elem_of_subseteq _ _)) ms_keys _ k_ms)=>k_keys.
+    destruct ((proj1 (elem_of_dom ms k)) k_ms) as (h & k_h).
+    iPoseProof (big_sepM_lookup_acc _ _ _ _ k_h with "cache") as
+        "((k_h & k_upd) & cache)".
+    wp_apply (SI_read_spec with "[//] k_h").
+    iIntros "k_h".
+    iSpecialize ("cache" with "[$k_h $k_upd]").
+    iAssert (∀ ms', ⌜dom ms = dom ms'⌝ -∗ P_tok -∗ (∀ m v0 h0,
+         ⌜dom m = dom ms⌝ ∗ φ m v0 h0 ∗ ConnectionState c (Active m) ∗
+         ([∗ map] k0↦h1 ∈ m, k0 ↦{ c} hist_val h1 ∗
+          KeyUpdStatus c k0 false) ∗ ([∗ map] k0↦h1 ∈ m, Seen k0 h1) -∗
+         Φ #()) -∗ ConnectionState c (Active ms') -∗ P -∗
+          ([∗ map] k0↦y ∈ ms', k0 ↦{ c} hist_val y ∗ KeyUpdStatus c k0 false) -∗
+       WP commitT c ;; 
+       snapshot_isolation_code.start c ;; 
+       (rec: "aux" <> :=
+          match: snapshot_isolation_code.read c #k with
+            InjL <> =>
+              commitT c ;; snapshot_isolation_code.start c ;; "aux" #()
+          | InjR "v" =>
+            if: cond "v" then commitT c ;; snapshot_isolation_code.start c
+            else commitT c ;; snapshot_isolation_code.start c ;; "aux" #()
+          end)%V #() @[ip_of_address sa] {{ v, Φ v }})%I as "retry".
+    {
+      iClear "Seen".
+      iIntros (ms') "%ms_ms' P_tok HΦ Active P cache".
+      wp_apply (commitT_spec with "[//]").
+      iPoseProof "inv" as "inv'".
+      iMod "inv'" as "(%m & %m_ms & mem & close)".
+      iModIntro.
+      iExists _, _, ((λ h, (hist_val h, false)) <$> ms').
+      iFrame.
+      iSplitL "cache".
+      {
+        iSplit.
+        {
+          iPureIntro.
+          rewrite bool_decide_spec=>k' k'_key.
+          rewrite lookup_fmap.
+          by case: (ms' !! k').
+        }
+        iSplit; first by rewrite m_ms.
+        iSplit; first by rewrite dom_fmap_L.
+        by iApply big_sepM_fmap.
+      }
+      iIntros "!>(CanStart & mem)".
+      iMod ("close" with "[mem]") as "_".
+      {
+        iPoseProof (big_sepM2_fmap_r _ _ _ ms' with "mem") as "mem".
+        iPoseProof (big_sepM2_sep with "mem") as "(mem & _)".
+        iPoseProof (big_sepM2_sep_2 (λ k h _, k ↦ₖ h)%I (λ _ _ _, emp)%I m ms'
+                with "[mem] []") as "mem".
+        {
+          iApply (big_sepM2_impl with "mem").
+          iIntros "!>%k' % %h' % %Hh' ?"=>{Hh'}.
+          by case: h'.
+        }
+        {
+          iApply big_sepM2_intro; last done.
+          move=>k'.
+          by split=>/(proj2 (elem_of_dom _ _)) Hk'; apply elem_of_dom;
+            [rewrite -ms_ms' -m_ms|rewrite m_ms ms_ms'].
+        }
+        iPoseProof (big_sepM2_sepM with "mem") as "(mem & _)"; last done.
+        move=>k'.
+        by split=>/(proj2 (elem_of_dom _ _)) Hk'; apply elem_of_dom;
+            [rewrite -ms_ms' -m_ms|rewrite m_ms ms_ms'].
+      }
+      iModIntro.
+      wp_pures.
+      wp_apply (SI_start_spec with "[//]").
+      iPoseProof "inv" as "inv'".
+      iClear (m m_ms) "".
+      iMod "inv'" as "(%m & %m_ms & mem & close)".
+      iModIntro.
+      iExists m.
+      iFrame.
+      iIntros "!>(Active & mem & cache & #Seen)".
+      iMod ("close" with "mem") as "_".
+      iModIntro.
+      wp_pures.
+      rewrite -m_ms.
+      by iApply ("IH" with
+          "P_tok [] [] inv finish cond_spec HΦ cache Active P Seen");
+        rewrite m_ms.
+    }
+    move: h k_h=>[|v' h] k_h. 
+    { wp_pures. iApply ("retry" with "[//] P_tok HΦ Active P cache"). }
+    wp_pures.
+    wp_apply ("cond_spec" with "[$P $Active $cache]"); first done.
+    iIntros (m []) "(Active & %m_ms & cache & result)"; last first.
+    {
+      wp_pures.
+      rewrite -m_ms.
+      by iApply ("retry" with "[] P_tok HΦ Active result cache").
+    }
+    iClear "IH retry cond_spec".
+    wp_pures.
+    wp_apply (commitT_spec with "[//]").
+    iPoseProof (big_sepM_lookup _ _ _ _ k_h with "Seen") as "#Seen_k".
+    iPoseProof "inv" as "inv'".
+    iMod "inv'" as "(%m' & %m'_ms & mem & close)".
+    iModIntro.
+    iExists _, _, ((λ h, (hist_val h, false)) <$> m).
+    iFrame.
+    iSplitL "cache".
+    {
+      iSplit.
+      {
+        iPureIntro.
+        rewrite bool_decide_spec=>k' k'_key.
+        rewrite lookup_fmap.
+        by case: (m !! k').
+      }
+      iSplit; first by rewrite m_ms.
+      iSplit; first by rewrite dom_fmap_L.
+      by iApply big_sepM_fmap.
+    }
+    iIntros "!>(CanStart & mem)".
+    iMod ("close" with "[mem]") as "_".
+    {
+      iPoseProof (big_sepM2_fmap_r _ _ _ m with "mem") as "mem".
+      iPoseProof (big_sepM2_sep with "mem") as "(mem & _)".
+      iPoseProof (big_sepM2_sep_2 (λ k h _, k ↦ₖ h)%I (λ _ _ _, emp)%I m' m
+              with "[mem] []") as "mem".
+      {
+        iApply (big_sepM2_impl with "mem").
+        iIntros "!>%k' % %h' % %Hh' ?"=>{Hh'}.
+        by case: h'.
+      }
+      {
+        iApply big_sepM2_intro; last done.
+        move=>k'.
+        by split=>/(proj2 (elem_of_dom _ _)) Hk'; apply elem_of_dom;
+          [rewrite m_ms -m'_ms|rewrite m'_ms -m_ms].
+      }
+      iPoseProof (big_sepM2_sepM with "mem") as "(mem & _)"; last done.
+      move=>k'.
+      by split=>/(proj2 (elem_of_dom _ _)) Hk'; apply elem_of_dom;
+          [rewrite m_ms -m'_ms|rewrite m'_ms -m_ms].
+    }
+    iModIntro.
+    wp_pures.
+    iClear (m m_ms m' m'_ms) "".
+    wp_apply (SI_start_spec with "[//]").
+    iMod ("finish" with "[$P_tok $result $Seen_k]") as "(%m & %m_ms &
+        mem & φ & Q_tok & close)".
+    iModIntro.
+    iExists m.
+    iFrame.
+    iIntros "!>(Active & mem & cache & #Seen')".
+    iMod ("close" with "[$mem $Q_tok]") as "_".
+    iApply "HΦ".
+    by iFrame "∗#%".
+  Qed.
+
+  Lemma simplified_wait_on_keyT_spec :
+    ∀ (c cond v : val) (k : Key) ms sa E φ P_tok Q_tok,
+    ⌜↑KVS_InvName ⊆ E⌝ -∗
+    ⌜dom ms ⊆ KVS_keys⌝ -∗
+    ⌜k ∈ dom ms⌝ -∗
+    □ (∀ h, Seen k (v :: h) ∗ P_tok ={⊤, E}=∗ ∃ m, ⌜dom m = dom ms⌝ ∗
+          ([∗ map] k ↦ h ∈ m, k ↦ₖ h) ∗ φ m ∗ Q_tok ∗ 
+              ▷ (([∗ map] k ↦ h ∈ m, k ↦ₖ h) ∗ Q_tok ={E, ⊤}=∗ emp)) -∗
+    □ (|={⊤, E}=> ∃ m, ⌜dom m = dom ms⌝ ∗ ([∗ map] k ↦ h ∈ m, k ↦ₖ h) ∗
+              ▷ (([∗ map] k ↦ h ∈ m, k ↦ₖ h) ={E, ⊤}=∗ emp)) -∗
+    (∀ v', {{{ True }}} cond v' @[ip_of_address sa]
+          {{{ (b : bool), RET #b; ⌜b → v = v'⌝ }}}) -∗
+    {{{
+      ConnectionState c (Active ms) ∗ P_tok ∗
+      ([∗ map] k ↦ h ∈ ms, k ↦{c} (hist_val h) ∗ KeyUpdStatus c k false) ∗
+      ([∗ map] k ↦ h ∈ ms, Seen k h)
+    }}}
+      wait_on_keyT c cond #k @[ip_of_address sa]
+    {{{ m, RET #(); ⌜dom m = dom ms⌝ ∗ φ m ∗
+      ConnectionState c (Active m) ∗
+      ([∗ map] k ↦ h ∈ m, k ↦{c} (hist_val h) ∗ KeyUpdStatus c k false) ∗
+      ([∗ map] k ↦ h ∈ m, Seen k h)
+    }}}.
+  Proof.
+    iIntros (cst cond v k ms sa E φ P_tok Q_tok name ms_keys k_ms)
+      "#finish #inv #cond_spec %Φ !> (Active & P_tok & cache & #Seen) HΦ".
+    iApply (wait_on_keyT_spec _ _ _ _ _ _ True P_tok (λ v', ⌜v = v'⌝)%I
+          (λ _ _ _, Q_tok) (λ m _ _, φ m) with "[//] [//] [//] [] inv []
+          [$P_tok $Active $cache $Seen] [HΦ]").
+    {
+      iIntros "!>% %h (P_tok & <- & #Seen')".
+      iApply ("finish" with "[$]").
+    }
+    {
+      iIntros (m v' Ψ) "!>(_ & Active & %m_ms & cache) HΨ".
+      wp_apply ("cond_spec" with "[//]").
+      iIntros (b v_v').
+      iApply ("HΨ" with "[$Active $cache]").
+      iSplit; first done.
+      by move: b v_v'=> [/(_ I)<-|].
+    }
+    iIntros "!>% % %".
+    iApply "HΦ".
+  Qed.
+
+End proof.
